Prove a top level correctness result (#37)
Refactor extraction into a new Extraction.v file that is sufficiently general to cover our use cases and prove a top level statement about it correct. To do this I had to

* Strengthen the erasure proof from MetaCoq to require only dependencies and not the whole environment to be erased.
* Change trans_env to translate type aliases into constants with boxes as bodies since these can appear in terms (although they should be removed later, we might want to prove that).
* Prove our recursive erasure procedure correct to be able to apply (1)
* Combine all the bits into a top level statement.

The top level statement is saying that any bool (in fact any constructor) that is not erasable will evaluate to the same constructor in the extracted environment.

extraction/theories/Erasure.v
@@ -12,6 +12,7 @@ From Equations Require Import Equations.
 From MetaCoq.Erasure Require Import EArities.
 From MetaCoq.Erasure Require Import Extract.
 From MetaCoq.Erasure Require Import Prelim.
+From MetaCoq.Erasure Require ErasureFunction.
 From MetaCoq.Erasure Require SafeErasureFunction.
 From MetaCoq.PCUIC Require Import PCUICAst.
 From MetaCoq.PCUIC Require Import PCUICAstUtils.
@@ -50,6 +51,11 @@ Import PCUICAst.
 
 Section FixSigmaExt.
 Local Existing Instance extraction_checker_flags.
+(* We abstract over the erasure func used since MetaCoq has both
+SafeErasureFunction and ErasureFunction. The former uses retyping, is
+computable within Coq and is generally better, but has fewer things
+proven about it and more axioms used. *)
+Context (erase_func : forall Σ, ∥wf_ext Σ∥ -> forall Γ t, welltyped Σ Γ t -> typing_result E.term).
 Context (Σ : global_env_ext).
 Context (wfextΣ : ∥wf_ext Σ∥).
 Let wfΣ : ∥wf Σ∥ := ltac:(now sq).
@@ -157,6 +163,7 @@ fot_viewc t := fot_view_other t _.
 Lemma watwf {Γ T} (wat : ∥isWfArity_or_Type Σ Γ T∥) : wellformed Σ Γ T.
 Proof. now apply wat_wellformed. Qed.
 
+Axiom needs_metacoq_proof : forall {A}, A.
 Equations(noeqns) flag_of_type (Γ : context) (T : term) (wat : ∥isWfArity_or_Type Σ Γ T∥)
   : typing_result (type_flag Γ T)
   by wf ((Γ;T; (watwf wat)) : (∑ Γ t, wellformed Σ Γ t)) term_rel :=
@@ -251,7 +258,7 @@ Next Obligation.
        the assumption that hnf of T is neither tProd nor tSort.
        To do this we will need to use some completeness fact about hnf,
        which is not proved in MetaCoq yet, so we defer this proof for now. *)
-    exact (todo "not an arity because of discr").
+    exact needs_metacoq_proof.
   - destruct isT as [[]].
     now econstructor.
 Qed.
@@ -263,10 +270,11 @@ Next Obligation.
   eapply validity; [easy|exact typK].
 Qed.
 Next Obligation.
-  exact (todo "also needs discr like above").
+  (* same as above *)
+  exact needs_metacoq_proof.
 Qed.
 Next Obligation.
-  exact (todo "also needs discr like above").
+  exact needs_metacoq_proof.
 Qed.
 
 Definition redβιζ : RedFlags.t :=
@@ -709,7 +717,7 @@ Program Definition erase_constant_decl
     et <- map_error EraseTypeError (erase_type [] []%vector (P.cst_type cst) _ []);;
     eb <- match P.cst_body cst with
          | Some body =>
-           match SafeErasureFunction.erase Σ wfextΣ [] body _ with
+           match erase_func Σ wfextΣ [] body _ with
            | TypeError te => Err (EraseBodyError te)
            | Checked eb => ret (Some eb)
            end
@@ -975,7 +983,7 @@ End FixSigmaExt.
 
 Section EraseEnv.
 Local Existing Instance extraction_checker_flags.
-Context (ignored : list kername).
+Context (erase_func : forall Σ, ∥wf_ext Σ∥ -> forall Γ t, welltyped Σ Γ t -> typing_result E.term).
 
 Import ExAst.
 
@@ -1003,44 +1011,16 @@ Program Definition erase_global_decl
   match decl with
   | P.ConstantDecl cst =>
     cst_or_ty_alias <- map_error (ErrConstant Σext kn)
-                                (erase_constant_decl Σext _ cst _);;
+                                 (erase_constant_decl erase_func Σext _ cst _);;
     match cst_or_ty_alias with
     | inl cst => ret (ConstantDecl cst)
     | inr ta => ret (TypeAliasDecl ta)
     end
   | P.InductiveDecl mib =>
     ind <- map_error (ErrInductive Σext kn)
-                     (erase_ind Σext _ kn mib _);;
+                     (erase_ind erase_func Σext _ kn mib _);;
     ret (InductiveDecl ignore_on_print ind)
   end.
-
-(* Erase all declarations for which [f] returns [true] *)
-Program Fixpoint general_erase_global_decls (Σ : P.global_env) (wfΣ : ∥wf Σ∥)
-        (f : kername -> bool)
-  : result global_env erase_global_decl_error :=
-  match Σ with
-  | [] => ret []
-  | (kn, decl) :: Σ =>
-    Σer <- general_erase_global_decls Σ _ f;;
-    if f kn then
-      ret Σer
-    else
-      let Σext := (Σ, universes_decl_of_decl decl) in
-      decl <- erase_global_decl Σext _ kn false decl _;;
-      ret ((kn, decl) :: Σer)
-  end.
-Next Obligation. now sq; inversion wfΣ. Qed.
-Next Obligation. now sq; inversion wfΣ. Qed.
-Next Obligation. now sq; inversion wfΣ. Qed.
-
-
-Definition contains (kn : kername) :=
-  List.existsb (eq_kername kn).
-
-(* Erase all unignored global declarations *)
-Definition erase_global_decls (Σ : P.global_env) (wfΣ : ∥wf Σ∥)
-  : result global_env erase_global_decl_error :=
-  general_erase_global_decls Σ wfΣ (fun kn => contains kn ignored).
 
 Definition add_seen (n : kername) (seen : list kername) : list kername :=
   if existsb (eq_kername n) seen then
@@ -1079,7 +1059,6 @@ Fixpoint box_type_deps (seen : list kername) (t : box_type) : list kername :=
   | TConst n => add_seen n seen
   end.
 
-
 Definition decl_deps (seen : list kername) (decl : global_decl) : list kername :=
   match decl with
   | ConstantDecl body =>
@@ -1105,12 +1084,6 @@ Definition is_inductive_decl (d : P.global_decl) : bool :=
   | P.InductiveDecl _ => true
   end.
 
-Definition Tis_inductive_decl (d : Ast.global_decl) : bool :=
-  match d with
-  | Ast.ConstantDecl _ => false
-  | Ast.InductiveDecl _ => true
-  end.
-
 (** Turn a global declaration into an axiom, if it's a constant, by removing the constant's body *)
 Definition decl_to_axiom (decl : global_decl) : global_decl :=
   match decl with
@@ -1124,13 +1097,17 @@ Definition decl_to_axiom (decl : global_decl) : global_decl :=
   | _ => decl
   end.
 
+Definition contains (kn : kername) :=
+  List.existsb (eq_kername kn).
 
-(* Erase the global declarations by the specified names and
-   their non-erased dependencies recursively. Ignore dependencies for which [ignore] returnes [true] *)
-Program Fixpoint general_erase_global_decls_deps_recursive
-        (Σ : P.global_env) (wfΣ : ∥wf Σ∥)
-        (ignore : kername -> bool)
+(* Erase the global declarations by the specified names and their
+   non-erased dependencies recursively. Ignore dependencies for which
+   [ignore] returnes [true] *)
+Program Fixpoint erase_global_decls_deps_recursive
+        (Σ : P.global_env)
+        (wfΣ : ∥wf Σ∥)
         (include : list kername)
+        (ignore : kername -> bool)
   : result global_env erase_global_decl_error :=
   match Σ with
   | [] => ret []
@@ -1138,85 +1115,42 @@ Program Fixpoint general_erase_global_decls_deps_recursive
     let Σext := (Σ, universes_decl_of_decl decl) in
     if contains kn include && negb (ignore kn)  then
       decl <- erase_global_decl Σext _ kn false decl _;;
-      Σer <- general_erase_global_decls_deps_recursive Σ _ ignore (decl_deps include decl);;
+      Σer <- erase_global_decls_deps_recursive Σ _ (decl_deps include decl) ignore;;
       ret ((kn, decl) :: Σer)
     else
       if contains kn include && ignore kn then
       (* NOTE: if the inductive declarations is ignored, we still add it to have enough info for printing [match] and inductives that depend on it. But we ignore its dependencies and ignore the declaration itself on printing *)
         decl <- erase_global_decl Σext _ kn true decl _;;
         let decl := decl_to_axiom decl in
-        Σer <- general_erase_global_decls_deps_recursive Σ _ ignore include ;;
+        Σer <- erase_global_decls_deps_recursive Σ _ include ignore ;;
         ret ((kn, decl) :: Σer)
-      else general_erase_global_decls_deps_recursive Σ _ ignore include
+      else
+        erase_global_decls_deps_recursive Σ _ include ignore
   end.
 Solve All Obligations with cbn;intros;subst; now sq; inversion wfΣ.
-
-(* Erase the unignored global declarations by the specified names and
-   their non-erased dependencies recursively. *)
-Program Fixpoint erase_global_decls_deps_recursive
-        (Σ : P.global_env) (wfΣ : ∥wf Σ∥)
-        (include : list kername)
-  : result global_env erase_global_decl_error :=
-  general_erase_global_decls_deps_recursive Σ wfΣ (fun kn => contains kn ignored) include.
-
-Fixpoint Tterm_deps (seen : list kername) (t : Ast.term) : list kername :=
-  match t with
-  | Ast.tRel _
-  | Ast.tVar _
-  | Ast.tSort _ => seen
-  | Ast.tCast t1 _ t2 => fold_left Tterm_deps [t1;t2] seen
-  | Ast.tInd ind _ => add_seen (inductive_mind ind) seen
-  | Ast.tProd _ ty1 ty2 => fold_left Tterm_deps [ty1;ty2] seen
-  | Ast.tEvar _ ts => fold_left Tterm_deps ts seen
-  | Ast.tLambda _ ty t => Tterm_deps seen t
-  | Ast.tLetIn _ ty t1 t2 => fold_left Tterm_deps [ty;t1;t2] seen
-  | Ast.tApp t1 t2 => fold_left Tterm_deps (t1 :: t2) seen
-  | Ast.tConst n _ => add_seen n seen
-  | Ast.tConstruct ind _ _ => add_seen (inductive_mind ind) seen
-  | Ast.tCase (ind, _) ty t brs =>
-    let seen := Tterm_deps (add_seen (inductive_mind ind) seen) t in
-    fold_left (fun seen '(_, t) => Tterm_deps seen t) brs seen
-  | Ast.tProj (ind, _, _) t => Tterm_deps (add_seen (inductive_mind ind) seen) t
-  | Ast.tFix defs _
-  | Ast.tCoFix defs _ =>
-    fold_left (fun seen d => Tterm_deps seen (BasicAst.dbody d)) defs seen
-  end.
-
-Definition Tdecl_deps (seen : list kername) (decl : Ast.global_decl) : list kername :=
-  match decl with
-  | Ast.ConstantDecl body =>
-    let seen :=
-        match Ast.cst_body body with
-        | Some body => Tterm_deps seen body
-        | None => seen
-        end in
-    Tterm_deps seen (Ast.cst_type body)
-  | Ast.InductiveDecl mib =>
-    let one_inductive_body_deps seen oib :=
-        let seen := fold_left Tterm_deps
-                              (map (snd ∘ fst) (Ast.ind_ctors oib))
-                              seen in
-        fold_left Tterm_deps (map snd (Ast.ind_projs oib)) seen in
-    fold_left one_inductive_body_deps (Ast.ind_bodies mib) seen
-  end.
-
-
-Import TemplateMonad.
-
-Program Fixpoint Tglobal_decls_deps_recursive
-        (Σ : Ast.global_env) (include : list kername)
-  : Ast.global_env :=
-  match Σ with
-  | [] => []
-  | (kn, decl) :: Σ =>
-    if contains kn include && negb (contains kn ignored) then
-        (kn, decl) :: Tglobal_decls_deps_recursive Σ (Tdecl_deps include decl)
-    else if Tis_inductive_decl decl && contains kn include && contains kn ignored then
-           (kn, decl) :: Tglobal_decls_deps_recursive Σ include
-         else Tglobal_decls_deps_recursive Σ include
-  end.
-
 End EraseEnv.
+
+(* Use SafeErasureFunction.erase for erasure. Runs from within Coq but has more
+   things admitted about it. *)
+Definition erase_global_decls_deps_recursive_safe_erasure :=
+  erase_global_decls_deps_recursive SafeErasureFunction.erase.
+
+Program Definition erase_with_normal_erasure
+        (cf := extraction_checker_flags)
+        (Σ : global_env_ext)
+        (wfΣ : ∥wf_ext Σ∥)
+        (Γ : context)
+        (t : term)
+        (wt : welltyped Σ Γ t) : typing_result E.term :=
+  ErasureFunction.erase Σ wfΣ Γ _ t.
+Next Obligation.
+  destruct wt.
+  sq.
+  now eapply typing_wf_local.
+Qed.
+
+Definition erase_global_decls_deps_recursive_normal_erasure :=
+  erase_global_decls_deps_recursive erase_with_normal_erasure.
 
 Global Arguments is_logical {_ _ _}.
 Global Arguments is_sort {_ _ _}.
