extraction/theories/OptimizeCorrectness.v
@@ -74,20 +74,23 @@ Definition trans_cst (cst : constant_body) : EAst.constant_body :=
 
 (* Translation from our global environment into MetaCoq's global environment.
    We only translate constants which is justified by the proof above. *)
-Definition trans (Σ : global_env) : EAst.global_context :=
+Definition trans_env (Σ : global_env) : EAst.global_context :=
   let map_decl kn (decl : global_decl) : list (kername * EAst.global_decl) :=
       match decl with
       | ConstantDecl cst => [(kn, EAst.ConstantDecl (trans_cst cst))]
       | InductiveDecl _ _ => []
-      | TypeAliasDecl _ => []
+      | TypeAliasDecl _ => [(kn, EAst.ConstantDecl {| EAst.cst_body := Some tBox |})]
       end in
   flat_map (fun '(kn, decl) => map_decl kn decl) Σ.
 
 Lemma declared_constant_trans Σ kn cst :
-  ETyping.declared_constant (trans Σ) kn cst ->
-  exists n typ,
+  ETyping.declared_constant (trans_env Σ) kn cst ->
+  (exists n typ,
     nth_error Σ n =
-    Some (kn, ConstantDecl {| cst_type := typ; cst_body := EAst.cst_body cst |}).
+    Some (kn, ConstantDecl {| cst_type := typ; cst_body := EAst.cst_body cst |})) \/
+  (EAst.cst_body cst = Some tBox /\
+    exists n typ,
+      nth_error Σ n = Some (kn, TypeAliasDecl typ)).
 Proof.
   unfold ETyping.declared_constant.
   intros decl.
@@ -96,14 +99,36 @@ Proof.
   - destruct (kername_eq_dec _ _) as [->|].
     + noconf decl.
       cbn in *.
-      exists 0, (cst_type c).
+      left.
+      eexists 0, (cst_type c).
       now destruct c.
-    + destruct IH as (n' & typ & cond); [assumption|].
+    + destruct IH as [(n' & typ & cond)|(isbox & n' & typ & cond)].
+      * eassumption.
+      * left.
+        now exists (S n'), typ.
+      * right.
+        split; [easy|].
+        now exists (S n'), typ.
+  - destruct IH as [(n' & typ & cond)|(isbox & n' & typ & cond)].
+    + eassumption.
+    + left.
       now exists (S n'), typ.
-  - destruct IH as (n' & typ & cond); [assumption|].
-    now exists (S n'), typ.
-  - destruct IH as (n' & typ & cond); [assumption|].
-    now exists (S n'), typ.
+    + right.
+      split; [easy|].
+      now exists (S n'), typ.
+  - destruct (kername_eq_dec _ _) as [->|].
+    + noconf decl.
+      cbn in *.
+      right.
+      split; [easy|].
+      now eexists 0, _.
+    + destruct IH as [(n' & typ & cond)|(isbox & n' & typ & cond)].
+      * eassumption.
+      * left.
+        now exists (S n'), typ.
+      * right.
+        split; [easy|].
+        now exists (S n'), typ.
 Qed.
 
 Fixpoint is_dead (rel : nat) (t : term) : bool :=
@@ -435,8 +460,7 @@ Lemma eval_dearg_lambdas_inv Σ mask Γ inner v :
   closed (it_mkLambda_or_LetIn Γ inner) ->
   #|mask| = #|vasses Γ| ->
   Σ ⊢ dearg_lambdas mask (it_mkLambda_or_LetIn Γ inner) ▷ v ->
-  ∑ tv,
-    Σ ⊢ it_mkLambda_or_LetIn Γ inner ▷ tv.
+  ∑ tv, Σ ⊢ it_mkLambda_or_LetIn Γ inner ▷ tv.
 Proof.
   intros env_clos clos len_eq ev.
   induction #|Γ| as [|Γlen IH] eqn:Γlen_eq in Γ, mask, inner, v, clos, len_eq, ev |- *.
@@ -893,6 +917,7 @@ Definition valid_masks_decl (p : kername * global_decl) : bool :=
   match p with
   | (kn, ConstantDecl {| cst_body := Some body |}) =>
     valid_dearg_mask (get_const_mask kn) body && valid_cases body
+  | (kn, TypeAliasDecl typ) => #|get_const_mask kn| =? 0
   | _ => true
   end.
 
@@ -1789,21 +1814,21 @@ Qed.
 
 Lemma is_expanded_constant Σ kn cst body :
   is_expanded_env Σ ->
-  ETyping.declared_constant (trans Σ) kn cst ->
+  ETyping.declared_constant (trans_env Σ) kn cst ->
   EAst.cst_body cst = Some body ->
   is_expanded body.
 Proof.
   intros exp_env decl body_eq.
   unfold is_expanded_env in *.
   apply forallb_Forall in exp_env.
-  eapply declared_constant_trans in decl as (? & ? & nth).
-  eapply nth_error_forall in nth; [|eassumption].
-  cbn in *.
-  now rewrite body_eq in nth.
+  eapply declared_constant_trans in decl as [(? & ? & nth)|(is_box & _)].
+  - rewrite body_eq in nth.
+    now eapply nth_error_forall in nth; [|eassumption].
+  - now replace body with tBox by congruence.
 Qed.
 
 Lemma eval_is_expanded_aux Σ t v k :
-  trans Σ ⊢ t ▷ v ->
+  trans_env Σ ⊢ t ▷ v ->
   is_expanded_env Σ ->
   is_expanded_aux k t ->
   is_expanded_aux k v .
@@ -2227,36 +2252,43 @@ Qed.
 
 Lemma valid_cases_constant Σ kn cst body :
   valid_masks_env Σ ->
-  ETyping.declared_constant (trans Σ) kn cst ->
+  ETyping.declared_constant (trans_env Σ) kn cst ->
   EAst.cst_body cst = Some body ->
   valid_cases body.
 Proof.
   intros valid_env decl_const body_eq.
-  eapply declared_constant_trans in decl_const as (? & ? & nth).
-  eapply nth_error_forallb in valid_env.
-  rewrite nth in valid_env.
-  cbn in *.
-  now rewrite body_eq in valid_env; propify.
+  eapply declared_constant_trans in decl_const as [(? & ? & nth)|(is_box & _)].
+  - eapply nth_error_forallb in valid_env.
+    rewrite nth in valid_env.
+    cbn in *.
+    now rewrite body_eq in valid_env; propify.
+  - now replace body with tBox by congruence.
 Qed.
 
 Lemma valid_dearg_mask_constant Σ kn cst body :
   valid_masks_env Σ ->
-  ETyping.declared_constant (trans Σ) kn cst ->
+  ETyping.declared_constant (trans_env Σ) kn cst ->
   EAst.cst_body cst = Some body ->
   valid_dearg_mask (get_const_mask kn) body.
 Proof.
   intros valid_env decl_const body_eq.
-  eapply declared_constant_trans in decl_const as (? & ? & nth).
-  eapply nth_error_forallb in valid_env.
-  rewrite nth in valid_env.
-  cbn in *.
-  now rewrite body_eq in valid_env; propify.
+  eapply declared_constant_trans in decl_const as [(? & ? & nth)|(is_box & ? & ? & nth)].
+  - eapply nth_error_forallb in valid_env.
+    rewrite nth in valid_env.
+    cbn in *.
+    now rewrite body_eq in valid_env; propify.
+  - eapply nth_error_forallb in valid_env.
+    rewrite nth in valid_env.
+    cbn in *.
+    replace body with tBox by congruence.
+    cbn.
+    now destruct get_const_mask.
 Qed.
 
 Lemma eval_valid_cases Σ t v :
-  trans Σ ⊢ t ▷ v ->
+  trans_env Σ ⊢ t ▷ v ->
 
-  env_closed (trans Σ) ->
+  env_closed (trans_env Σ) ->
   closed t ->
 
   valid_masks_env Σ ->
@@ -2347,9 +2379,9 @@ Proof with auto with dearg.
 Qed.
 
 Lemma declared_constant_dearg Σ k cst :
-  ETyping.declared_constant (trans Σ) k cst ->
+  ETyping.declared_constant (trans_env Σ) k cst ->
   ∑ cst',
-    ETyping.declared_constant (trans (dearg_env Σ)) k cst' ×
+    ETyping.declared_constant (trans_env (dearg_env Σ)) k cst' ×
     EAst.cst_body cst' = option_map (dearg ∘ dearg_lambdas (get_const_mask k))
                                     (EAst.cst_body cst).
 Proof.
@@ -2364,7 +2396,11 @@ Proof.
       now split; [reflexivity|].
     + now apply IH.
   - now apply IH.
-  - now apply IH.
+  - destruct (kername_eq_dec k kn) as [->|].
+    + noconf typ.
+      eexists.
+      now split; [reflexivity|].
+    + now apply IH.
 Qed.
 
 Inductive dearg_spec : term -> term -> Type :=
@@ -2626,16 +2662,16 @@ Ltac facts :=
 Section dearg.
   Context (n : nat).
   Context (Σ : global_env).
-  Context (clos_Σ : env_closed (trans Σ)).
+  Context (clos_Σ : env_closed (trans_env Σ)).
   Context (valid_Σ : valid_masks_env Σ).
   Context (exp_Σ : is_expanded_env Σ).
   Context (IH : forall t v : term,
         closed t ->
         valid_cases t ->
         is_expanded t ->
-        forall ev : trans Σ ⊢ t ▷ v,
+        forall ev : trans_env Σ ⊢ t ▷ v,
         deriv_length ev <= n ->
-        trans (dearg_env Σ) ⊢ dearg t ▷ dearg v).
+        trans_env (dearg_env Σ) ⊢ dearg t ▷ dearg v).
 
   Lemma eval_tApp_dearg {hd arg v} :
     closed hd ->
@@ -2645,9 +2681,9 @@ Section dearg.
     closed arg ->
     valid_cases arg ->
     is_expanded arg ->
-    forall (ev : trans Σ ⊢ tApp hd arg ▷ v),
+    forall (ev : trans_env Σ ⊢ tApp hd arg ▷ v),
       deriv_length ev <= S n ->
-      trans (dearg_env Σ) ⊢ tApp (dearg hd) (dearg arg) ▷ dearg v.
+      trans_env (dearg_env Σ) ⊢ tApp (dearg hd) (dearg arg) ▷ dearg v.
   Proof with auto with dearg.
     intros clos_hd valid_hd exp_hd clos_arg valid_arg exp_arg ev ev_len.
     depind ev; cbn in *.
@@ -2754,9 +2790,9 @@ Section dearg.
     Forall (closedn 0) args ->
     Forall valid_cases args ->
     Forall is_expanded args ->
-    forall (ev : trans Σ ⊢ mkApps hd args ▷ v),
+    forall (ev : trans_env Σ ⊢ mkApps hd args ▷ v),
       deriv_length ev <= n ->
-      trans (dearg_env Σ) ⊢ mkApps (dearg hd) (map dearg args) ▷ dearg v.
+      trans_env (dearg_env Σ) ⊢ mkApps (dearg hd) (map dearg args) ▷ dearg v.
   Proof.
     intros clos_hd valid_hd exp_hd clos_args valid_args exp_args ev ev_len.
     pose proof (eval_mkApps_deriv ev) as (hdv & ev_hd & argsv & ev_args & ev_args_len).
@@ -2789,10 +2825,10 @@ Section dearg.
     Forall (closedn 0) args ->
     Forall valid_cases args ->
     Forall is_expanded args ->
-    (args = [] -> trans (dearg_env Σ) ⊢ dearg hd ▷ dearg v) ->
-    forall (ev : trans Σ ⊢ mkApps hd args ▷ v),
+    (args = [] -> trans_env (dearg_env Σ) ⊢ dearg hd ▷ dearg v) ->
+    forall (ev : trans_env Σ ⊢ mkApps hd args ▷ v),
       deriv_length ev <= S n ->
-      trans (dearg_env Σ) ⊢ mkApps (dearg hd) (map dearg args) ▷ dearg v.
+      trans_env (dearg_env Σ) ⊢ mkApps (dearg hd) (map dearg args) ▷ dearg v.
   Proof.
     intros clos_hd valid_hd exp_hd clos_args valid_args exp_args no_args ev ev_len.
     destruct args as [|? ? _] using MCList.rev_ind; cbn in *; [easy|].
@@ -2834,8 +2870,8 @@ Section dearg.
 End dearg.
 
 Lemma env_closed_dearg Σ :
-  env_closed (trans Σ) ->
-  env_closed (trans (dearg_env Σ)).
+  env_closed (trans_env Σ) ->
+  env_closed (trans_env (dearg_env Σ)).
 Proof.
   intros clos.
   induction Σ as [|(kn & decl) Σ IH]; [easy|].
@@ -2938,7 +2974,7 @@ Proof.
 Qed.
 
 Lemma dearg_correct Σ t v :
-  env_closed (trans Σ) ->
+  env_closed (trans_env Σ) ->
   closed t ->
 
   valid_masks_env Σ ->
@@ -2947,13 +2983,13 @@ Lemma dearg_correct Σ t v :
   is_expanded_env Σ ->
   is_expanded t ->
 
-  trans Σ ⊢ t ▷ v ->
-  trans (dearg_env Σ) ⊢ dearg t ▷ dearg v.
+  trans_env Σ ⊢ t ▷ v ->
+  trans_env (dearg_env Σ) ⊢ dearg t ▷ dearg v.
 Proof.
   intros clos_env clos_t valid_env valid_t exp_env exp_t.
-  enough (forall n (ev : trans Σ ⊢ t ▷ v),
+  enough (forall n (ev : trans_env Σ ⊢ t ▷ v),
              deriv_length ev <= n ->
-             trans (dearg_env Σ) ⊢ dearg t ▷ dearg v).
+             trans_env (dearg_env Σ) ⊢ dearg t ▷ dearg v).
   { intros ev.
     eapply (H _ ev).
     apply le_refl. }
@@ -2968,7 +3004,7 @@ Proof.
     destruct isdecl_dearg as (cst_dearg & decl_dearg & body_dearg).
     rewrite e in body_dearg; cbn in *.
 
-    enough (trans (dearg_env Σ)
+    enough (trans_env (dearg_env Σ)
             ⊢ dearg_single (get_const_mask kn)
                            (dearg (dearg_lambdas (get_const_mask kn) body))
                            (map dearg args) ▷ dearg v) as ev'.
@@ -2980,7 +3016,7 @@ Proof.
 
     rewrite dearg_dearg_lambdas by
         eauto using valid_dearg_mask_constant, valid_cases_constant.
-    assert (∑ ev' : trans Σ ⊢ mkApps body args ▷ v,
+    assert (∑ ev' : trans_env Σ ⊢ mkApps body args ▷ v,
                deriv_length ev' < deriv_length ev) as (ev_body & deriv_body).
     { unshelve epose proof (eval_mkApps_heads_deriv _ ev_const ev) as (ev' & ?).
       - now econstructor.
@@ -3020,7 +3056,7 @@ Proof.
     apply is_expanded_aux_mkApps_inv in exp_t as (exp_hd & exp_args).
     cbn in *; propify.
     rewrite !dearg_single_masked by (now rewrite map_length).
-    assert (ev_args_dearg: All2 (eval (trans (dearg_env Σ))) (map dearg args) (map dearg argsv)).
+    assert (ev_args_dearg: All2 (eval (trans_env (dearg_env Σ))) (map dearg args) (map dearg argsv)).
     { assert (all_smaller: sum_deriv_lengths ev_args <= n).
       { pose proof (deriv_length_min ev_constr).
         lia. }
@@ -3372,25 +3408,21 @@ Proof.
         -- lia.
     + destruct t; cbn in *; try destruct y; try congruence; now constructor.
 Qed.
-
-Lemma metacoq_dearg_correct Σ t v :
-  env_closed (trans Σ) ->
-  closed t ->
-
-  valid_masks_env Σ ->
-  valid_cases t ->
-
-  is_expanded_env Σ ->
-  is_expanded t ->
-
-  trans Σ p⊢ t ▷ v ->
-  trans (dearg_env Σ) p⊢ dearg t ▷ dearg v.
-Proof.
-  intros ? ? ? ? ? ? ev.
-  apply eval_evalT in ev as [ev].
-  apply evalT_eval.
-  now apply dearg_correct.
-Qed.
 End dearg_correct.
 
 Print Assumptions dearg_correct.
+
+Lemma trans_env_debox_env_types Σ :
+  trans_env (debox_env_types Σ) = trans_env Σ.
+Proof.
+  unfold debox_env_types.
+  generalize Σ at 1 as masks.
+  induction Σ as [|(kn, decl) Σ IH]; intros masks; [easy|].
+  cbn in *.
+  destruct decl; cbn in *.
+  - f_equal.
+    apply IH.
+  - easy.
+  - f_equal.
+    apply IH.
+Qed.
