extraction/examples/StackInterpreter.v
@@ -151,7 +151,7 @@ Definition INTERP_MODULE : LiquidityMod params _ _ storage action :=
     that removes application of boxes to constants and constructors. *)
 
 Time MetaCoq Run
-     (t <- liquitidy_extraction PREFIX TT_remap TT_rename INTERP_MODULE ;;
+     (t <- liquidity_extraction PREFIX TT_remap TT_rename INTERP_MODULE ;;
       tmDefinition INTERP_MODULE.(lmd_module_name) t
      ).
 
