extraction/theories/ErasureCorrectness.v
@@ -1,0 +1,858 @@
+From ConCert.Extraction Require Import ClosedAux.
+From ConCert.Extraction Require Import Erasure.
+From ConCert.Extraction Require Import Extraction.
+From ConCert.Extraction Require Import MetaCoqErasureCorrectnessStrong.
+From ConCert.Extraction Require Import Optimize.
+From ConCert.Extraction Require Import OptimizeCorrectness.
+From ConCert.Extraction Require Import ResultMonad.
+From ConCert.Extraction Require Import WcbvEvalType.
+From Coq Require Import List.
+From Coq Require Import Permutation.
+From Coq Require Import String.
+From Equations Require Import Equations.
+From MetaCoq.Erasure Require Import ErasureCorrectness.
+From MetaCoq.Erasure Require Import ErasureFunction.
+From MetaCoq.Erasure Require Import ESubstitution.
+From MetaCoq.Erasure Require Import EWcbvEval.
+From MetaCoq.Erasure Require Import Extract.
+From MetaCoq.PCUIC Require Import PCUICAstUtils.
+From MetaCoq.PCUIC Require Import PCUICInduction.
+From MetaCoq.PCUIC Require Import PCUICInversion.
+From MetaCoq.PCUIC Require Import PCUICSafeLemmata.
+From MetaCoq.PCUIC Require Import PCUICSR.
+From MetaCoq.PCUIC Require Import PCUICTyping.
+From MetaCoq.PCUIC Require Import PCUICWcbvEval.
+From MetaCoq.PCUIC Require Import PCUICWeakeningEnv.
+From MetaCoq.Template Require Import BasicAst.
+From MetaCoq.Template Require Import utils.
+
+Open Scope string.
+
+Import ListNotations.
+
+Module P := PCUICAst.
+Module E := EAst.
+
+Notation "Σ 'p⊢' s ▷ t" := (PCUICWcbvEval.eval Σ s t) (at level 50, s, t at next level) : type_scope.
+Notation "Σ 'e⊢' s ▷ t" := (EWcbvEval.eval Σ s t) (at level 50, s, t at next level) : type_scope.
+
+Lemma contains_In k ks :
+  Erasure.contains k ks <-> In k ks.
+Proof.
+  split; intros.
+  - unfold contains in *.
+    apply existsb_exists in H as (? & ? & ?).
+    unfold eq_kername in *.
+    now destruct kername_eq_dec as [<-|].
+  - unfold contains.
+    induction ks; cbn in *; [easy|].
+    destruct H as [->|].
+    + now rewrite eq_kername_refl.
+    + rewrite IHks by easy.
+      now rewrite Bool.orb_true_r.
+Qed.
+
+Lemma contains_In_not k ks :
+  Erasure.contains k ks = false <-> ~ In k ks.
+Proof.
+  split; intros.
+  - intros isin.
+    now apply contains_In in isin.
+  - destruct (contains k ks) eqn:cont; [|easy].
+    now apply contains_In in cont.
+Qed.
+
+Lemma erases_deps_forall_ind Σ Σ'
+  (P : Extract.E.term -> Prop)
+  (Hbox : P Extract.E.tBox)
+  (Hrel : forall i : nat, P (Extract.E.tRel i))
+  (Hvar : forall n : ident, P (Extract.E.tVar n))
+  (Hevar :
+     forall (m : nat) (l : list Extract.E.term),
+       Forall P l ->
+       Forall (erases_deps Σ Σ') l -> P (Extract.E.tEvar m l))
+  (Hlam : forall (na : name) (body : Extract.E.term),
+        erases_deps Σ Σ' body -> P body -> P (Extract.E.tLambda na body))
+  (Hletin : forall (na : name) (val body : Extract.E.term),
+        erases_deps Σ Σ' val ->
+        P val -> erases_deps Σ Σ' body -> P body -> P (Extract.E.tLetIn na val body))
+  (Happ : forall hd arg : Extract.E.term,
+        erases_deps Σ Σ' hd -> P hd -> erases_deps Σ Σ' arg -> P arg -> P (Extract.E.tApp hd arg))
+  (Hconst : forall (kn : kername) (cb : PCUICAst.PCUICEnvironment.constant_body) (cb' : EAst.constant_body),
+      declared_constant Σ kn cb ->
+      ETyping.declared_constant Σ' kn cb' ->
+      erases_constant_body (Σ, PCUICAst.cst_universes cb) cb cb' ->
+      (forall body : Extract.E.term, Extract.E.cst_body cb' = Some body -> erases_deps Σ Σ' body) ->
+      (forall body : Extract.E.term, Extract.E.cst_body cb' = Some body -> P body) ->
+        P (Extract.E.tConst kn))
+  (Hconstruct : forall (ind : inductive) (c : nat), P (Extract.E.tConstruct ind c))
+  (Hcase : forall (p : inductive × nat) (discr : Extract.E.term) (brs : list (nat × Extract.E.term)),
+        erases_deps Σ Σ' discr ->
+        P discr ->
+        Forall (fun br : nat × Extract.E.term => erases_deps Σ Σ' br.2) brs ->
+        Forall (fun br => P br.2) brs ->
+        P (Extract.E.tCase p discr brs))
+  (Hproj : forall (p : projection) (t : Extract.E.term),
+        erases_deps Σ Σ' t -> P t -> P (Extract.E.tProj p t))
+  (Hfix : forall (defs : list (Extract.E.def Extract.E.term)) (i : nat),
+         Forall (fun d : Extract.E.def Extract.E.term => erases_deps Σ Σ' (Extract.E.dbody d)) defs ->
+         Forall (fun d => P (E.dbody d)) defs ->
+         P (Extract.E.tFix defs i))
+  (Hcofix : forall (defs : list (Extract.E.def Extract.E.term)) (i : nat),
+         Forall (fun d : Extract.E.def Extract.E.term => erases_deps Σ Σ' (Extract.E.dbody d)) defs ->
+         Forall (fun d => P (E.dbody d)) defs ->
+         P (Extract.E.tCoFix defs i)) :
+  forall t, erases_deps Σ Σ' t -> P t.
+Proof.
+  fix f 2.
+  intros t ed.
+  move f at top.
+  destruct ed;
+    try solve [match goal with
+    | [H: _ |- _] => apply H
+    end; auto].
+  - apply Hevar; [|assumption].
+    revert l H.
+    fix f' 2.
+    intros l [].
+    + now constructor.
+    + constructor; [now apply f|now apply f'].
+  - eapply Hconst; try eassumption.
+    intros.
+    apply f.
+    now apply H2.
+  - apply Hcase; try assumption.
+    + now apply f.
+    + revert brs H.
+      fix f' 2.
+      intros brs []; [now constructor|].
+      constructor; [now apply f|now apply f'].
+  - apply Hfix; try assumption.
+    revert defs H.
+    fix f' 2.
+    intros defs []; [now constructor|].
+    constructor; [now apply f|now apply f'].
+  - apply Hcofix; try assumption.
+    revert defs H.
+    fix f' 2.
+    intros defs []; [now constructor|].
+    constructor; [now apply f|now apply f'].
+Defined.
+
+Lemma erases_deps_cons_left Σ Σ' kn decl t :
+  wf ((kn, decl) :: Σ) ->
+  erases_deps Σ Σ' t ->
+  erases_deps ((kn, decl) :: Σ) Σ' t.
+Proof.
+  intros wfΣ er.
+  induction er using erases_deps_forall_ind; try solve [now constructor].
+  apply lookup_env_Some_fresh in H as not_fresh.
+  econstructor.
+  - unfold declared_constant in *.
+    cbn.
+    unfold eq_kername.
+    inversion wfΣ; subst.
+    destruct kername_eq_dec as [<-|]; [congruence|].
+    eassumption.
+  - eassumption.
+  - unfold erases_constant_body in *.
+    destruct PCUICAst.cst_body eqn:body.
+    + destruct E.cst_body eqn:ebody; [|easy].
+      assert (declared_constant ((kn, decl) :: Σ) kn0 cb).
+      { unfold declared_constant.
+        cbn.
+        unfold eq_kername.
+        inversion wfΣ; subst.
+        destruct kername_eq_dec as [<-|]; [congruence|].
+        easy. }
+      inversion wfΣ; subst.
+      eapply PCUICWeakeningEnv.declared_constant_inv in H4; eauto.
+      2:eapply PCUICWeakeningEnv.weaken_env_prop_typing.
+      red in H4.
+      rewrite body in *.
+      cbn in *.
+      eapply (erases_extends (_, P.cst_universes cb)); eauto.
+      2: eexists [_]; reflexivity.
+      eapply declared_constant_inv in H.
+      2:eapply PCUICWeakeningEnv.weaken_env_prop_typing.
+      2: easy.
+      2: easy.
+      unfold on_constant_decl in H.
+      rewrite body in *.
+      apply H.
+    + now destruct E.cst_body.
+  - easy.
+Qed.
+
+Lemma erases_deps_cons Σ Σ' kn decl decl' t :
+  wf ((kn, decl) :: Σ) ->
+  erases_deps Σ Σ' t ->
+  erases_deps ((kn, decl) :: Σ) ((kn, decl') :: Σ') t.
+Proof.
+  intros wfΣ er.
+  induction er using erases_deps_forall_ind; try solve [now constructor].
+  apply lookup_env_Some_fresh in H as not_fresh.
+  econstructor.
+  - unfold declared_constant in *.
+    cbn.
+    unfold eq_kername.
+    inversion wfΣ; subst.
+    destruct kername_eq_dec as [<-|]; [congruence|].
+    eassumption.
+  - unfold ETyping.declared_constant in *.
+    cbn.
+    inversion wfΣ; subst.
+    destruct kername_eq_dec; [congruence|].
+    eassumption.
+  - unfold erases_constant_body in *.
+    destruct PCUICAst.cst_body eqn:body.
+    + destruct E.cst_body eqn:ebody; [|easy].
+      assert (declared_constant ((kn, decl) :: Σ) kn0 cb).
+      { unfold declared_constant.
+        cbn.
+        unfold eq_kername.
+        inversion wfΣ; subst.
+        destruct kername_eq_dec as [<-|]; [congruence|].
+        easy. }
+      inversion wfΣ; subst.
+      eapply PCUICWeakeningEnv.declared_constant_inv in H4; eauto.
+      2:eapply PCUICWeakeningEnv.weaken_env_prop_typing.
+      red in H4.
+      rewrite body in *.
+      cbn in *.
+      eapply (erases_extends (_, P.cst_universes cb)); eauto.
+      2: eexists [_]; reflexivity.
+      eapply declared_constant_inv in H.
+      2:eapply PCUICWeakeningEnv.weaken_env_prop_typing.
+      2: easy.
+      2: easy.
+      unfold on_constant_decl in H.
+      rewrite body in *.
+      apply H.
+    + now destruct E.cst_body.
+  - easy.
+Qed.
+
+Lemma In_add_seen k k' ks :
+  (k = k' \/ In k ks) ->
+  In k (add_seen k' ks).
+Proof.
+  intros [->|].
+  - unfold add_seen.
+    destruct existsb eqn:ex; [|now left].
+    apply existsb_exists in ex as (k & ? & ?).
+    unfold eq_kername in *.
+    now destruct kername_eq_dec as [<-|].
+  - unfold add_seen.
+    destruct existsb eqn:ex; [easy|].
+    now right.
+Qed.
+
+Lemma In_box_type_deps k ks t :
+  In k ks ->
+  In k (box_type_deps ks t).
+Proof.
+  intros isin.
+  induction t in ks, t, isin |- *; cbn in *; auto.
+  - now apply In_add_seen.
+  - now apply In_add_seen.
+Qed.
+
+Lemma In_fold_left {A} k (ks : list kername) f (ts : list A) :
+  In k ks ->
+  (forall a ks, In a ts -> In k ks -> In k (f ks a)) ->
+  In k (fold_left f ts ks).
+Proof.
+  intros isin allin.
+  induction ts in ks, ts, isin, allin |- *; [easy|].
+  apply IHts.
+  - apply allin; [|easy].
+    now left.
+  - intros.
+    apply allin; [|easy].
+    now right.
+Qed.
+
+Lemma In_Eterm_deps_already k ks t :
+  In k ks ->
+  In k (Eterm_deps ks t).
+Proof.
+  intros isin.
+  induction t in ks, t, isin |- * using EInduction.term_forall_list_ind; cbn in *; auto.
+  - induction H in ks, isin |- *; [easy|].
+    cbn in *.
+    now apply IHForall.
+  - now apply In_add_seen.
+  - now apply In_add_seen.
+  - destruct p.
+    apply In_fold_left.
+    + now apply IHt, In_add_seen.
+    + intros.
+      destruct a.
+      now eapply All_In in H as [H]; [|eassumption].
+  - destruct s as ((ind & npars) & arg).
+    now apply IHt, In_add_seen.
+  - apply In_fold_left; [easy|].
+    intros.
+    now eapply Forall_All, All_In in H as [H]; [|eassumption].
+  - apply In_fold_left; [easy|].
+    intros.
+    now eapply Forall_All, All_In in H as [H]; [|eassumption].
+Qed.
+
+Lemma In_fold_left_new_exists {A} k (ks : list kername) f (ts : list A) :
+  In k (fold_left f ts ks) ->
+  ~In k ks ->
+  exists tspref t' tssuf,
+    ts = (tspref ++ [t'] ++ tssuf)%list /\
+    ~In k (fold_left f tspref ks) /\
+    In k (f (fold_left f tspref ks) t').
+Proof.
+  intros isin notin.
+  induction ts in ks, ts, isin, notin |- *; cbn in *; [congruence|].
+  destruct (contains k (f ks a)) eqn:cont.
+  - apply contains_In in cont.
+    now exists [], a, ts.
+  - apply IHts in isin as (pref & t' & suf & -> & ? & ?); cycle 1.
+    { intros isin'.
+      apply contains_In in isin'.
+      congruence. }
+    now exists (a :: pref), t', suf.
+Qed.
+
+Lemma In_fold_left_new {A} k (ks ks' : list kername) f (ts : list A) :
+  In k (fold_left f ts ks) ->
+  ~In k ks ->
+  (forall a ks, In a ts -> In k ks -> In k (f ks a)) ->
+  (forall a ks ks', In a ts -> ~In k ks -> In k (f ks a) -> In k (f ks' a)) ->
+  In k (fold_left f ts ks').
+Proof.
+  intros isin notin allin_already allin_new.
+  destruct (In_fold_left_new_exists _ _ _ _ isin) as (tspref & t' & tssuf & -> & ? & ?); [easy|].
+  rewrite !fold_left_app in *.
+  cbn in *.
+  apply In_fold_left.
+  - eapply allin_new; [| |exact H0].
+    + apply in_or_app.
+      now right; left.
+    + easy.
+  - intros.
+    eapply allin_already; [|easy].
+    apply in_or_app.
+    now right; right.
+Qed.
+
+Lemma add_seen_new k ks k' :
+  ~In k ks ->
+  In k (add_seen k' ks) ->
+  k = k'.
+Proof.
+  intros notin isin.
+  unfold add_seen in *.
+  destruct existsb eqn:ex; [easy|].
+  now destruct isin.
+Qed.
+
+Lemma In_Eterm_deps_new k ks ks' t :
+  In k (Eterm_deps ks t) ->
+  ~In k ks ->
+  In k (Eterm_deps ks' t).
+Proof.
+  intros isin notin.
+  induction t in ks, ks', isin, notin |- * using EInduction.term_forall_list_ind; cbn in *; try easy.
+  - eapply In_fold_left_new; eauto.
+    + intros.
+      now apply In_Eterm_deps_already.
+    + intros.
+      now eapply Forall_All, All_In in H as [H]; [|eassumption].
+  - destruct (contains k (Eterm_deps ks t1)) eqn:cont.
+    + apply contains_In in cont.
+      now apply In_Eterm_deps_already.
+    + eapply IHt2; [easy|].
+      apply contains_In_not.
+      eassumption.
+  - destruct (contains k (Eterm_deps ks t1)) eqn:cont.
+    + apply contains_In in cont.
+      now apply In_Eterm_deps_already.
+    + eapply IHt2; [easy|].
+      apply contains_In_not.
+      eassumption.
+  - apply add_seen_new in isin as ->; [|easy].
+    now apply In_add_seen.
+  - apply add_seen_new in isin as ->; [|easy].
+    now apply In_add_seen.
+  - destruct p.
+    destruct (contains k (Eterm_deps (add_seen (inductive_mind i) ks) t)) eqn:cont.
+    + apply contains_In in cont.
+      apply In_fold_left.
+      * destruct (eq_dec k (inductive_mind i)) as [->|].
+        -- now apply In_Eterm_deps_already, In_add_seen.
+        -- eapply IHt; [eassumption|].
+           intros isin'.
+           now apply add_seen_new in isin'; subst.
+      * intros; destruct a.
+        now apply In_Eterm_deps_already.
+    + apply contains_In_not in cont.
+      eapply In_fold_left_new; eauto.
+      * intros; destruct a.
+        now apply In_Eterm_deps_already.
+      * intros; destruct a.
+        now eapply All_In in X as []; [|eassumption].
+  - destruct s as ((? & ?) & ?).
+    destruct (eq_dec (inductive_mind i) k) as [<-|].
+    + now apply In_Eterm_deps_already, In_add_seen.
+    + eapply IHt; [easy|].
+      intros isin'.
+      now apply add_seen_new in isin'; subst.
+  - eapply In_fold_left_new; eauto.
+    + intros.
+      now apply In_Eterm_deps_already.
+    + intros.
+      now eapply Forall_All, All_In in H as [H]; [|eassumption].
+  - eapply In_fold_left_new; eauto.
+    + intros.
+      now apply In_Eterm_deps_already.
+    + intros.
+      now eapply Forall_All, All_In in H as [H]; [|eassumption].
+Qed.
+
+Lemma In_fold_box_type_deps k ks ts :
+  In k ks ->
+  In k (fold_left box_type_deps ts ks).
+Proof.
+  intros isin.
+  induction ts in ks, ts, isin |- *; [easy|].
+  now apply IHts, In_box_type_deps.
+Qed.
+
+Lemma In_decl_deps k ks decl :
+  In k ks ->
+  In k (decl_deps ks decl).
+Proof.
+  intros isin.
+  destruct decl; cbn in *.
+  - apply In_box_type_deps.
+    destruct ExAst.cst_body; [|easy].
+    now apply In_Eterm_deps_already.
+  - apply In_fold_left; [easy|].
+    intros.
+    apply In_fold_left.
+    + apply In_fold_left; [easy|].
+      intros.
+      now eapply In_box_type_deps.
+    + intros.
+      now apply In_box_type_deps.
+  - destruct p.
+    now apply In_box_type_deps.
+Qed.
+
+Lemma erases_forall_list_ind
+      Σ (P : P.context -> P.term -> E.term -> Prop)
+(Hrel : forall (Γ : P.context) (i : nat), P Γ (P.tRel i) (E.tRel i))
+(Hvar : forall (Γ : P.context) (n : ident), P Γ (P.tVar n) (E.tVar n))
+(Hevar : forall (Γ : P.context) (m m' : nat) (l : list P.term) (l' : list E.term),
+ All2 (erases Σ Γ) l l' ->
+ Forall2 (P Γ) l l' ->
+ P Γ (P.tEvar m l) (E.tEvar m' l'))
+(Hlam : forall (Γ : P.context) (na : name) (b t : P.term) (t' : E.term),
+ Σ;;; (P.vass na b :: Γ) |- t ⇝ℇ t' ->
+ P (P.vass na b :: Γ) t t' -> P Γ (P.tLambda na b t) (E.tLambda na t'))
+(Hletin : forall (Γ : P.context) (na : name) (t1 : P.term) (t1' : E.term)
+   (T t2 : P.term) (t2' : E.term),
+ Σ;;; Γ |- t1 ⇝ℇ t1' ->
+ P Γ t1 t1' ->
+ Σ;;; (P.vdef na t1 T :: Γ) |- t2 ⇝ℇ t2' ->
+ P (P.vdef na t1 T :: Γ) t2 t2' ->
+ P Γ (P.tLetIn na t1 T t2) (E.tLetIn na t1' t2'))
+(Happ : forall (Γ : P.context) (f4 u : P.term) (f' u' : E.term),
+ Σ;;; Γ |- f4 ⇝ℇ f' ->
+ P Γ f4 f' -> Σ;;; Γ |- u ⇝ℇ u' -> P Γ u u' -> P Γ (P.tApp f4 u) (E.tApp f' u'))
+(Hconst : forall (Γ : P.context) (kn : kername) (u : Universes.Instance.t),
+ P Γ (P.tConst kn u) (E.tConst kn))
+(Hconstruct : forall (Γ : P.context) (kn : inductive) (k : nat) (n : Universes.Instance.t),
+ P Γ (P.tConstruct kn k n) (E.tConstruct kn k))
+(Hcase : forall (Γ : P.context) (ind : inductive) (npar : nat) (T c : P.term)
+   (brs : list (nat × P.term)) (c' : E.term) (brs' : list (nat × E.term)),
+ PCUICElimination.Informative Σ ind ->
+ Σ;;; Γ |- c ⇝ℇ c' ->
+ P Γ c c' ->
+ All2
+   (fun (x : nat × P.term) (x' : nat × E.term) => Σ;;; Γ |- x.2 ⇝ℇ x'.2 × x.1 = x'.1)
+   brs brs' ->
+Forall2 (fun br br' => P Γ br.2 br'.2) brs brs' ->
+ P Γ (P.tCase (ind, npar) T c brs) (E.tCase (ind, npar) c' brs'))
+(Hproj : forall (Γ : P.context) (p : (inductive × nat) × nat) (c : P.term)
+   (c' : E.term),
+ let ind := p.1.1 in
+ PCUICElimination.Informative Σ ind ->
+ Σ;;; Γ |- c ⇝ℇ c' -> P Γ c c' -> P Γ (P.tProj p c) (E.tProj p c'))
+(Hfix : forall (Γ : P.context) (mfix : mfixpoint P.term) (n : nat)
+   (mfix' : list (E.def E.term)),
+ All2
+   (fun (d : def P.term) (d' : E.def E.term) =>
+    dname d = E.dname d'
+    × rarg d = E.rarg d'
+      × Σ;;; P.app_context Γ (PCUICLiftSubst.fix_context mfix) |-
+        dbody d ⇝ℇ E.dbody d') mfix mfix' ->
+ Forall2 (fun d d' => P (P.app_context Γ (PCUICLiftSubst.fix_context mfix)) (dbody d) (EAst.dbody d') ) mfix mfix' ->
+ P Γ (P.tFix mfix n) (E.tFix mfix' n))
+(Hcofix : forall (Γ : P.context) (mfix : mfixpoint P.term) (n : nat)
+   (mfix' : list (E.def E.term)),
+ All2
+   (fun (d : def P.term) (d' : E.def E.term) =>
+    dname d = E.dname d'
+    × rarg d = E.rarg d'
+      × Σ;;; P.app_context Γ (PCUICLiftSubst.fix_context mfix) |-
+        dbody d ⇝ℇ E.dbody d') mfix mfix' ->
+ Forall2 (fun d d' => P (P.app_context Γ (PCUICLiftSubst.fix_context mfix)) (dbody d) (EAst.dbody d') ) mfix mfix' ->
+ P Γ (P.tCoFix mfix n) (E.tCoFix mfix' n))
+(Hbox : forall (Γ : P.context) (t : P.term), isErasable Σ Γ t -> P Γ t E.tBox) :
+  forall (Γ : P.context) (t : P.term) (t0 : E.term),
+    Σ;;; Γ |- t ⇝ℇ t0 -> P Γ t t0.
+Proof.
+  fix f 4.
+  intros Γ t et er.
+  move f at top.
+  destruct er;
+    try solve [match goal with
+    | [H: _ |- _] => apply H
+    end; auto].
+  - apply Hevar; [assumption|].
+    revert l l' X.
+    fix f' 3.
+    intros l l' [].
+    + now constructor.
+    + constructor; [now apply f|now apply f'].
+  - apply Hcase; try assumption.
+    + now apply f.
+    + revert brs brs' X.
+      fix f' 3.
+      intros brs brs' []; [now constructor|].
+      constructor; [now apply f|now apply f'].
+  - apply Hfix; try assumption.
+    revert X.
+    generalize mfix at 1 3.
+    intros mfix_gen.
+    revert mfix mfix'.
+    fix f' 3.
+    intros mfix mfix' []; [now constructor|].
+    constructor; [now apply f|now apply f'].
+  - apply Hcofix; try assumption.
+    revert X.
+    generalize mfix at 1 3.
+    intros mfix_gen.
+    revert mfix mfix'.
+    fix f' 3.
+    intros mfix mfix' []; [now constructor|].
+    constructor; [now apply f|now apply f'].
+Defined.
+
+Lemma erases_deps_recursive Σ Σer t T et :
+  wf_ext Σ ->
+  Σ;;; [] |- t : T ->
+  Σ;;; [] |- t ⇝ℇ et ->
+  (forall k,
+      In k (Eterm_deps [] et) ->
+      match P.lookup_env Σ k with
+      | Some (P.ConstantDecl _) => erases_deps Σ Σer (E.tConst k)
+      | _ => True
+      end) ->
+  erases_deps Σ Σer et.
+Proof.
+  intros wf wt er deps_er.
+  induction er in t, T, et, wf, wt, er, deps_er |- * using erases_forall_list_ind; cbn in *.
+  - now constructor.
+  - now constructor.
+  - now apply inversion_Evar in wt.
+  - constructor.
+    apply inversion_Lambda in wt as (? & ? & ? & ? & ?); eauto.
+  - apply inversion_LetIn in wt as (? & ? & ? & ? & ? & ?); eauto.
+    constructor.
+    + eapply IHer1; eauto.
+      intros.
+      apply deps_er.
+      now apply In_Eterm_deps_already.
+    + eapply IHer2; eauto.
+      intros.
+      apply deps_er.
+      now eapply In_Eterm_deps_new.
+  - apply inversion_App in wt as (? & ? & ? & ? & ? & ?); eauto.
+    constructor.
+    + eapply IHer1; eauto.
+      intros.
+      apply deps_er.
+      now apply In_Eterm_deps_already.
+    + eapply IHer2; eauto.
+      intros.
+      apply deps_er.
+      now eapply In_Eterm_deps_new.
+  - apply inversion_Const in wt as (? & ? & ? & ? & ?); eauto.
+    specialize (deps_er kn (or_introl eq_refl)).
+    unfold declared_constant in d.
+    unfold PCUICAst.fst_ctx, fst_ctx in *.
+    now rewrite d in deps_er.
+  - now constructor.
+  - apply inversion_Case in wt
+      as (? & ? & ? & ? & ? & ? & ? & ? & ? & ? & ? & ? & ? & ? & ? & ? & ?); eauto.
+    constructor.
+    + eapply IHer; eauto.
+      intros.
+      eapply deps_er.
+      eapply In_fold_left.
+      * now eapply In_Eterm_deps_new.
+      * intros.
+        destruct a0.
+        now apply In_Eterm_deps_already.
+    + clear -wf a X H0 deps_er.
+      revert brs' x5 a X H0 deps_er.
+      induction brs; intros brs' x5 brtys typ er deps.
+      { now depelim er. }
+      depelim brtys.
+      depelim typ.
+      depelim er.
+      destruct p as ((? & ?) & ?).
+      destruct p0.
+      constructor.
+      * eapply H; eauto.
+        intros.
+        apply deps.
+        cbn.
+        destruct y0; cbn in *.
+        apply In_fold_left.
+        -- now eapply In_Eterm_deps_new.
+        -- intros; destruct a0.
+           now apply In_Eterm_deps_already.
+      * eapply IHbrs; eauto.
+        intros.
+        apply deps.
+        cbn.
+        destruct y0; cbn in *.
+        destruct (contains k (Eterm_deps (Eterm_deps [inductive_mind ind] c') t1)) eqn:cont.
+        -- apply contains_In in cont.
+           apply In_fold_left; cbn in *; [easy|].
+           intros; destruct a0.
+           now apply In_Eterm_deps_already.
+        -- apply contains_In_not in cont.
+           eapply In_fold_left_new; eauto.
+           ++ intros isin'.
+              contradiction cont.
+              now apply In_Eterm_deps_already.
+           ++ intros; destruct a0.
+              now apply In_Eterm_deps_already.
+           ++ intros; destruct a0.
+              eapply In_Eterm_deps_new; eauto.
+
+  - apply inversion_Proj in wt as (?&?&?&?&?&?&?&?&?); eauto.
+    constructor.
+    eapply IHer; eauto.
+    intros; apply deps_er.
+    destruct p as ((? & ?) & ?).
+    now eapply In_Eterm_deps_new.
+  - constructor.
+    apply inversion_Fix in wt as (?&?&?&?&?&?&?); eauto.
+    clear -wf a0 X H deps_er.
+    revert a0 X H deps_er.
+    generalize mfix at 1 2 4 6.
+    intros mfix_gen.
+    revert mfix'.
+    induction mfix; cbn in *; intros mfix' typ er all_deps deps.
+    { now depelim er. }
+    depelim typ.
+    depelim er.
+    depelim all_deps.
+    destruct p.
+    destruct p0 as (?&?&?).
+    constructor.
+    + eapply H; eauto.
+      intros.
+      apply deps.
+      cbn in *.
+      apply In_fold_left; [easy|].
+      intros.
+      now apply In_Eterm_deps_already.
+    + apply IHmfix; eauto.
+      intros.
+      apply deps.
+      cbn in *.
+      eapply In_fold_left_new; eauto.
+      * intros.
+        now apply In_Eterm_deps_already.
+      * intros.
+        now eapply In_Eterm_deps_new.
+  - constructor.
+    apply inversion_CoFix in wt as (?&?&?&?&?&?&?); eauto.
+    clear -wf a0 X H deps_er.
+    revert a0 X H deps_er.
+    generalize mfix at 1 2 4 6.
+    intros mfix_gen.
+    revert mfix'.
+    induction mfix; cbn in *; intros mfix' typ er all_deps deps.
+    { now depelim er. }
+    depelim typ.
+    depelim er.
+    depelim all_deps.
+    destruct p as (?&?&?).
+    constructor.
+    + eapply H; eauto.
+      intros.
+      apply deps.
+      cbn in *.
+      apply In_fold_left; [easy|].
+      intros.
+      now apply In_Eterm_deps_already.
+    + apply IHmfix; eauto.
+      intros.
+      apply deps.
+      cbn in *.
+      eapply In_fold_left_new; eauto.
+      * intros.
+        now apply In_Eterm_deps_already.
+      * intros.
+        now eapply In_Eterm_deps_new.
+  - now constructor.
+Qed.
+
+Opaque erase_type SafeErasureFunction.wf_reduction.
+Lemma erase_global_decls_deps_recursive_correct Σ wfΣ include ignore erase_func Σex :
+  (forall k, ignore k = false) ->
+  (forall Σ Γ t T wfΣ t',
+      Σ;;; Γ |- t : T ->
+      forall wt,
+        erase_func Σ wfΣ Γ t wt = PCUICSafeChecker.Checked t' ->
+        Σ;;; Γ |- t ⇝ℇ t') ->
+  erase_global_decls_deps_recursive erase_func Σ wfΣ include ignore = Ok Σex ->
+  (forall k,
+      In k include ->
+      match P.lookup_env Σ k with
+      | Some (P.ConstantDecl cst) =>
+        erases_deps Σ (trans_env Σex) (E.tConst k)
+      | _ => True
+      end).
+Proof.
+  intros no_ignores erase_erases er.
+  induction Σ as [|(kn, decl) Σ IH] in wfΣ, include, Σex, er |- *; [easy|].
+  cbn in *.
+  match goal with
+  | [H: context[erase_global_decl _ _ ?wfΣarg _ _ _ ?wfdeclarg] |- _] =>
+      set (wfΣext := wfΣarg) in *; clearbody wfΣext;
+        set (wfdecl := wfdeclarg) in *; clearbody wfdecl
+  end.
+  match goal with
+  | [H: context[erase_global_decls_deps_recursive _ _ ?wfΣarg] |- _] =>
+    set (wfΣprev := wfΣarg) in *; clearbody wfΣprev
+  end.
+
+  rewrite no_ignores in er.
+  destruct (contains kn include) eqn:contains; cycle 1.
+  - cbn in *.
+    intros.
+    eapply IH with (k := k) in er; eauto.
+    unfold eq_kername.
+    destruct kername_eq_dec as [->|].
+    + now apply contains_In in H.
+    + destruct P.lookup_env; [|easy].
+      destruct g; [|easy].
+      destruct wfΣ.
+      now apply erases_deps_cons_left.
+  - cbn in *.
+    destruct erase_global_decl eqn:erdecl; cbn in *; [|congruence].
+    destruct erase_global_decls_deps_recursive eqn:errec; [|congruence].
+    inversion er; subst; clear er.
+    intros k isin.
+    unfold eq_kername.
+    destruct kername_eq_dec as [->|]; cycle 1.
+    { cbn in *.
+      eapply IH with (k := k) in errec; eauto.
+      destruct P.lookup_env; [|easy].
+      destruct g; [|easy].
+      destruct wfΣ.
+      destruct t;
+        eauto using erases_deps_cons, erases_deps_cons_left.
+      now apply In_decl_deps. }
+    destruct decl; [|easy].
+    cbn -[erase_constant_decl] in *.
+    destruct erase_constant_decl eqn:erconst; cbn -[erase_constant_decl] in *; [|congruence].
+    unfold erase_constant_decl in erconst.
+    destruct flag_of_type; cbn in *; [|congruence].
+    destruct a; cbn in *.
+    destruct is_sort.
+    + cbn in wfdecl.
+      destruct c.
+      destruct cst_body; cbn in *; [|congruence].
+      destruct erase_type; cbn in *; [|congruence].
+      inversion erconst; subst; clear erconst.
+      inversion erdecl; subst; clear erdecl.
+      cbn in *.
+      econstructor.
+      * unfold declared_constant; cbn; rewrite eq_kername_refl.
+        reflexivity.
+      * unfold ETyping.declared_constant; cbn.
+        destruct kername_eq_dec; [|congruence].
+        reflexivity.
+      * cbn.
+        destruct wfΣ as [wfΣ].
+        destruct wfdecl as [wfdecl].
+        destruct i as (u & [redu]).
+        eapply type_reduction in wfdecl; eauto.
+        2: now inversion wfΣ.
+        constructor.
+        eapply (Is_type_extends (Σ, _)).
+        2: now eauto.
+        2: eexists [_]; reflexivity.
+        1: now eauto.
+        eexists _.
+        split; [eassumption|].
+        now left.
+      * intros.
+        cbn in *.
+        inversion H; subst; clear H.
+        now constructor.
+    + destruct erase_type; cbn in *; [|congruence].
+      destruct c; cbn in *.
+      destruct cst_body; cycle 1.
+      { inversion erconst; subst; clear erconst.
+        inversion erdecl; subst; clear erdecl.
+        cbn in *.
+        econstructor.
+        - unfold declared_constant; cbn; rewrite eq_kername_refl; reflexivity.
+        - unfold ETyping.declared_constant; cbn.
+          destruct kername_eq_dec; [|congruence].
+          reflexivity.
+        - easy.
+        - intros.
+          cbn in *.
+          congruence. }
+
+      destruct erase_func eqn:er; cbn in *; [|congruence].
+      inversion erconst; subst; clear erconst.
+      inversion erdecl; subst; clear erdecl.
+      cbn in *.
+      specialize (IH _ _ _ errec).
+      destruct wfΣ as [wfΣ].
+      destruct wfdecl as [wfdecl].
+      eapply erase_erases in er; eauto.
+      econstructor.
+      * unfold declared_constant; cbn; rewrite eq_kername_refl; reflexivity.
+      * unfold ETyping.declared_constant; cbn.
+        destruct kername_eq_dec; [|congruence].
+        reflexivity.
+      * cbn.
+        eapply type_reduction in wfdecl; eauto.
+        2: now inversion wfΣ.
+        eapply (erases_extends (_, _)).
+        2: eauto.
+        1: now inversion wfΣ.
+        2: eexists [_]; reflexivity.
+        2: eauto.
+        eauto.
+      * intros.
+        cbn in *.
+        noconf H.
+        destruct wfΣext.
+        apply erases_deps_cons; eauto.
+        eapply (erases_deps_recursive (Σ, cst_universes)); eauto.
+        intros.
+        apply IH.
+        apply In_box_type_deps.
+        now eapply In_Eterm_deps_new.
+Qed.
