extraction/theories/ExtractionCorrectness.v
@@ -1,0 +1,117 @@
+From ConCert.Extraction Require Import Aux.
+From ConCert.Extraction Require Import ClosedAux.
+From ConCert.Extraction Require Import Erasure.
+From ConCert.Extraction Require Import ErasureCorrectness.
+From ConCert.Extraction Require Import Extraction.
+From ConCert.Extraction Require Import MetaCoqErasureCorrectnessStrong.
+From ConCert.Extraction Require Import Optimize.
+From ConCert.Extraction Require Import OptimizeCorrectness.
+From ConCert.Extraction Require Import ResultMonad.
+From ConCert.Extraction Require Import WcbvEvalType.
+From Coq Require Import Arith.
+From Coq Require Import List.
+From Coq Require Import String.
+From Equations Require Import Equations.
+From MetaCoq.Erasure Require Import ErasureFunction.
+From MetaCoq.Erasure Require Import EWcbvEval.
+From MetaCoq.Erasure Require Import Extract.
+From MetaCoq.Erasure Require Import Prelim.
+From MetaCoq.PCUIC Require Import PCUICAstUtils.
+From MetaCoq.PCUIC Require Import PCUICSafeLemmata.
+From MetaCoq.PCUIC Require Import PCUICTyping.
+From MetaCoq.PCUIC Require PCUICWcbvEval.
+From MetaCoq.Template Require Import BasicAst.
+From MetaCoq.Template Require Import utils.
+
+Open Scope string.
+
+Import ListNotations.
+
+Module P := PCUICAst.
+Module E := EAst.
+
+Notation "Σ 'p⊢' s ▷ t" := (PCUICWcbvEval.eval Σ s t) (at level 50, s, t at next level) : type_scope.
+Notation "Σ 'e⊢' s ▷ t" := (EWcbvEval.eval Σ s t) (at level 50, s, t at next level) : type_scope.
+
+Lemma eval_const_construct_mask Σ kn ind c im cm :
+  trans_env Σ e⊢ E.tConst kn ▷ E.tConstruct ind c ->
+  valid_masks_env im cm Σ ->
+  get_const_mask cm kn = [].
+Proof.
+  intros ev valid.
+  depelim ev.
+  unfold valid_masks_env in valid.
+  apply forallb_Forall in valid.
+  apply declared_constant_trans in isdecl as [(? & ? & nth)|(isbox & ? & ? & nth)]; cycle 1.
+  { eapply nth_error_forall in nth; [|eassumption].
+    cbn in *.
+    now destruct get_const_mask. }
+  eapply nth_error_forall in nth; [|eassumption].
+  cbn in *.
+  rewrite H in nth.
+  propify.
+  destruct nth as (valid_mask_body & _).
+  clear -ev valid_mask_body.
+  enough (#|get_const_mask cm kn| = 0) by (now destruct get_const_mask).
+  apply valid_dearg_mask_spec in valid_mask_body as (Γ & inner & <- & <-).
+  induction #|Γ| as [|Γlen IH] eqn:eq in Γ, inner, ev |- *.
+  - now destruct Γ.
+  - destruct Γ as [|[na [body|]] Γ]; cbn in *.
+    + easy.
+    + depelim ev.
+      refold.
+      rewrite subst_it_mkLambda_or_LetIn in ev2.
+      erewrite <- vasses_subst_context.
+      eapply IH; [eassumption|].
+      now rewrite length_subst_context.
+    + depelim ev.
+Qed.
+
+Theorem extract_correct (Σ : P.global_env_ext) kn ui ind c ui' (wfΣ : wf_ext Σ) exΣ :
+  axiom_free Σ ->
+  welltyped Σ [] (P.tConst kn ui) ->
+  Σ p⊢ P.tConst kn ui ▷ P.tConstruct ind c ui' ->
+  (isErasable Σ [] (P.tConstruct ind c ui') -> False) ->
+  extract_pcuic_env
+    (pcuic_params check_masks_args)
+    Σ (wf_ext_wf_squash wfΣ) [kn] (fun _ => false) = Ok exΣ ->
+  trans_env exΣ e⊢ E.tConst kn ▷ E.tConstruct ind c.
+Proof.
+  intros ax [T wt] ev not_erasable ex.
+  cbn in *.
+  destruct erase_global_decls_deps_recursive as [Σex|] eqn:er; cbn in *; [|congruence].
+  destruct env_closed eqn:closed; cbn in *; [|congruence].
+  destruct analyze_env eqn:an; cbn in *.
+  destruct is_expanded_env eqn:isexp; cbn in *; [|congruence].
+  destruct valid_masks_env eqn:valid; cbn in *; [|congruence].
+  inversion_clear ex.
+  rewrite trans_env_debox_env_types.
+  eapply erase_global_decls_deps_recursive_correct in er; eauto.
+  3: left; reflexivity.
+  2: intros.
+  2: now eapply SafeErasureFunction.erases_erase.
+  assert (ev' := ev).
+  depelim ev'.
+  unfold declared_constant in isdecl.
+  rewrite isdecl in er.
+
+  eapply erases_correct in er as (erv & erase_to & erev); eauto.
+  2: now constructor.
+
+  depelim erase_to; [|easy].
+
+  eapply eval_const_construct_mask in erev as no_mask; eauto.
+  apply eval_evalT in erev as [erev].
+  assert (ctor_exp := erev).
+  eapply eval_is_expanded_aux with (k := 0) in ctor_exp; eauto.
+  2: now cbn; rewrite no_mask.
+  cbn in *.
+  eapply dearg_correct in erev; eauto.
+  - cbn in *.
+    rewrite no_mask in erev.
+    destruct get_ctor_mask; [|easy].
+    cbn in *.
+    now apply evalT_eval.
+  - cbn.
+    now rewrite no_mask.
+Qed.
