extraction/theories/MetaCoqErasureCorrectnessStrong.v
@@ -1,0 +1,1075 @@
+(* This file copies the erasure correctness proof from MetaCoq and
+   strengthens it for our use where where we do not erase full
+   environments but rather only dependencies.
+   The admitted proofs in this file comes from the MetaCoq development. *)
+
+From Coq Require Import Bool String List Program.Basics Program.Tactics ZArith.
+From MetaCoq.Template Require Import config utils monad_utils.
+From MetaCoq.Erasure Require Import ELiftSubst ETyping EWcbvEval Extract Prelim
+     ESubstitution EInversion EArities ErasureCorrectness.
+From MetaCoq.PCUIC Require Import PCUICTyping PCUICAst PCUICAstUtils
+  PCUICWeakening PCUICSubstitution PCUICArities
+  PCUICWcbvEval PCUICSR  PCUICInversion
+  PCUICUnivSubstitution PCUICElimination PCUICCanonicity
+  PCUICUnivSubst PCUICWeakeningEnv PCUICCumulativity.
+From ConCert.Extraction Require Import Aux.
+
+Require Import ssreflect.
+Require Import Equations.Prop.DepElim.
+
+Local Open Scope string_scope.
+Set Asymmetric Patterns.
+Local Set Keyed Unification.
+
+Import MonadNotation.
+
+Require Import Lia.
+
+Module PA := PCUICAst.
+Module P := PCUICWcbvEval.
+
+Local Existing Instance config.extraction_checker_flags.
+
+Hint Resolve wf_ext_wk_wf : core.
+Hint Resolve Is_type_conv_context : core.
+
+Transparent PCUICParallelReductionConfluence.construct_cofix_discr.
+
+Import E.
+Inductive erases_deps (Σ : PA.global_env) (Σ' : global_declarations) : term -> Prop :=
+| erases_deps_tBox : erases_deps Σ Σ' tBox
+| erases_deps_tRel i : erases_deps Σ Σ' (tRel i)
+| erases_deps_tVar n : erases_deps Σ Σ' (tVar n)
+| erases_deps_tEvar m l :
+    Forall (erases_deps Σ Σ') l ->
+    erases_deps Σ Σ' (tEvar m l)
+| erases_deps_tLambda na body :
+    erases_deps Σ Σ' body ->
+    erases_deps Σ Σ' (tLambda na body)
+| erases_deps_tLetIn na val body :
+    erases_deps Σ Σ' val ->
+    erases_deps Σ Σ' body ->
+    erases_deps Σ Σ' (tLetIn na val body)
+| erases_deps_tApp hd arg :
+    erases_deps Σ Σ' hd ->
+    erases_deps Σ Σ' arg ->
+    erases_deps Σ Σ' (tApp hd arg)
+| erases_deps_tConst kn cb cb' :
+    PCUICTyping.declared_constant Σ kn cb ->
+    ETyping.declared_constant Σ' kn cb' ->
+    erases_constant_body (Σ, cst_universes cb) cb cb' ->
+    (forall body, cst_body cb' = Some body -> erases_deps Σ Σ' body) ->
+    erases_deps Σ Σ' (tConst kn)
+| erases_deps_tConstruct ind c :
+    erases_deps Σ Σ' (tConstruct ind c)
+| erases_deps_tCase p discr brs :
+    erases_deps Σ Σ' discr ->
+    Forall (fun br => erases_deps Σ Σ' br.2) brs ->
+    erases_deps Σ Σ' (tCase p discr brs)
+| erases_deps_tProj p t :
+    erases_deps Σ Σ' t ->
+    erases_deps Σ Σ' (tProj p t)
+| erases_deps_tFix defs i :
+    Forall (fun d => erases_deps Σ Σ' (dbody d)) defs ->
+    erases_deps Σ Σ' (tFix defs i)
+| erases_deps_tCoFix defs i :
+    Forall (fun d => erases_deps Σ Σ' (dbody d)) defs ->
+    erases_deps Σ Σ' (tCoFix defs i).
+
+Derive Signature for erases_deps.
+Derive Signature for Forall.
+
+Lemma erases_deps_mkApps Σ Σ' hd args :
+  erases_deps Σ Σ' hd ->
+  Forall (erases_deps Σ Σ') args ->
+  erases_deps Σ Σ' (mkApps hd args).
+Proof.
+  intros er erall.
+  induction args using rev_ind; [easy|].
+  rewrite !emkApps_snoc.
+  apply Forall_app in erall as (? & ?).
+  depelim H0.
+  now constructor.
+Qed.
+
+Lemma erases_deps_mkApps_inv Σ Σ' hd args :
+  erases_deps Σ Σ' (mkApps hd args) ->
+  erases_deps Σ Σ' hd /\ Forall (erases_deps Σ Σ') args.
+Proof.
+  intros er.
+  induction args using rev_ind; [easy|].
+  rewrite -> emkApps_snoc in *.
+  depelim er.
+  intuition auto.
+  now apply Forall_app_inv.
+Qed.
+
+Lemma erases_deps_lift Σ Σ' n k t :
+  erases_deps Σ Σ' t ->
+  erases_deps Σ Σ' (lift n k t).
+Proof.
+  intros er.
+  induction t in k, t, er |- * using EInduction.term_forall_list_ind; cbn in *; auto.
+  - now destruct (_ <=? _); constructor.
+  - depelim er.
+    constructor.
+    induction H; cbn in *; [easy|].
+    now depelim H0.
+  - depelim er.
+    now constructor.
+  - depelim er.
+    now constructor.
+  - depelim er.
+    now constructor.
+  - depelim er.
+    constructor; [easy|].
+    induction X; [easy|].
+    depelim H.
+    constructor; [|easy].
+    now cbn.
+  - depelim er.
+    now constructor.
+  - depelim er.
+    constructor.
+    induction H in k, H, H0 |- *; [easy|].
+    cbn in *.
+    rewrite <- !Nat.add_succ_r.
+    depelim H0.
+    constructor; [|easy].
+    now apply H.
+  - depelim er.
+    constructor.
+    induction H in k, H, H0 |- *; [easy|].
+    cbn in *.
+    rewrite <- !Nat.add_succ_r.
+    depelim H0.
+    constructor; [|easy].
+    now apply H.
+Qed.
+
+Lemma erases_deps_subst Σ Σ' s k t :
+  All (erases_deps Σ Σ') s ->
+  erases_deps Σ Σ' t ->
+  erases_deps Σ Σ' (subst s k t).
+Proof.
+  intros aller er.
+  induction t in k, aller, er |- * using EInduction.term_forall_list_ind; cbn in *; auto.
+  - destruct (_ <=? _); [|now constructor].
+    destruct nth_error eqn:nth; [|now constructor].
+    eapply All_nth_error in nth; [|now eauto].
+    now apply erases_deps_lift.
+  - depelim er.
+    constructor.
+    induction H; [easy|].
+    depelim H0.
+    now constructor.
+  - depelim er.
+    now constructor.
+  - depelim er.
+    now constructor.
+  - depelim er.
+    now constructor.
+  - depelim er.
+    constructor; [easy|].
+    induction X; [easy|].
+    depelim H.
+    constructor; [|easy].
+    now cbn.
+  - depelim er.
+    now constructor.
+  - depelim er.
+    constructor.
+    induction H in k, H, H0 |- *; [easy|].
+    cbn in *.
+    rewrite <- !Nat.add_succ_r.
+    depelim H0.
+    constructor; [|easy].
+    now apply H.
+  - depelim er.
+    constructor.
+    induction H in k, H, H0 |- *; [easy|].
+    cbn in *.
+    rewrite <- !Nat.add_succ_r.
+    depelim H0.
+    constructor; [|easy].
+    now apply H.
+Qed.
+
+Lemma erases_deps_subst1 Σ Σ' t k u :
+  erases_deps Σ Σ' t ->
+  erases_deps Σ Σ' u ->
+  erases_deps Σ Σ' (subst1 t k u).
+Proof.
+  intros.
+  apply erases_deps_subst; [|easy].
+  now constructor.
+Qed.
+
+Lemma erases_deps_csubst Σ Σ' s k t :
+  erases_deps Σ Σ' s ->
+  erases_deps Σ Σ' t ->
+  erases_deps Σ Σ' (ECSubst.csubst s k t).
+Proof.
+  intros aller er.
+  induction t in k, aller, er |- * using EInduction.term_forall_list_ind; cbn in *; auto.
+  - destruct (_ ?= _); try constructor; easy.
+  - depelim er.
+    constructor.
+    induction H; [easy|].
+    depelim H0.
+    now constructor.
+  - depelim er.
+    now constructor.
+  - depelim er.
+    now constructor.
+  - depelim er.
+    now constructor.
+  - depelim er.
+    constructor; [easy|].
+    induction X; [easy|].
+    depelim H.
+    constructor; [|easy].
+    now cbn.
+  - depelim er.
+    now constructor.
+  - depelim er.
+    constructor.
+    induction H in k, H, H0 |- *; [easy|].
+    cbn in *.
+    rewrite <- !Nat.add_succ_r.
+    depelim H0.
+    constructor; [|easy].
+    now apply H.
+  - depelim er.
+    constructor.
+    induction H in k, H, H0 |- *; [easy|].
+    cbn in *.
+    rewrite <- !Nat.add_succ_r.
+    depelim H0.
+    constructor; [|easy].
+    now apply H.
+Qed.
+
+Lemma erases_deps_substl Σ Σ' s t :
+  Forall (fun s => erases_deps Σ Σ' s) s ->
+  erases_deps Σ Σ' t ->
+  erases_deps Σ Σ' (Ee.substl s t).
+Proof.
+  intros all exp.
+  unfold Ee.substl.
+  induction s using List.rev_ind; [easy|].
+  rewrite fold_left_app.
+  cbn.
+  apply Forall_snoc in all.
+  now apply erases_deps_csubst.
+Qed.
+
+Lemma Forall_erases_deps_fix_subst Σ Σ' defs :
+  Forall (erases_deps Σ Σ' ∘ dbody) defs ->
+  Forall (erases_deps Σ Σ') (ETyping.fix_subst defs).
+Proof.
+  intros all.
+  unfold ETyping.fix_subst.
+  induction defs at 2; constructor; cbn in *.
+  - now constructor.
+  - now apply IHl.
+Qed.
+
+Lemma Forall_erases_deps_cofix_subst Σ Σ' defs :
+  Forall (erases_deps Σ Σ' ∘ dbody) defs ->
+  Forall (erases_deps Σ Σ') (ETyping.cofix_subst defs).
+Proof.
+  intros all.
+  unfold ETyping.cofix_subst.
+  induction defs at 2; constructor; cbn in *.
+  - now constructor.
+  - now apply IHl.
+Qed.
+
+Lemma erases_deps_cunfold_fix Σ Σ' defs i narg f :
+  Ee.cunfold_fix defs i = Some (narg, f) ->
+  Forall (fun d => erases_deps Σ Σ' (dbody d)) defs ->
+  erases_deps Σ Σ' f.
+Proof.
+  intros cuf all.
+  unfold Ee.cunfold_fix in *.
+  destruct (nth_error _ _) eqn:nth; [|congruence].
+  eapply nth_error_forall in nth; [|eassumption].
+  noconf cuf.
+  apply erases_deps_substl; [|easy].
+  now apply Forall_erases_deps_fix_subst.
+Qed.
+
+Lemma erases_deps_cunfold_cofix Σ Σ' defs i narg f :
+  Ee.cunfold_cofix defs i = Some (narg, f) ->
+  Forall (fun d => erases_deps Σ Σ' (dbody d)) defs ->
+  erases_deps Σ Σ' f.
+Proof.
+  intros cuf all.
+  unfold Ee.cunfold_cofix in *.
+  destruct (nth_error _ _) eqn:nth; [|congruence].
+  eapply nth_error_forall in nth; [|eassumption].
+  noconf cuf.
+  apply erases_deps_substl; [|easy].
+  now apply Forall_erases_deps_cofix_subst.
+Qed.
+
+Lemma erases_deps_fix_subst Σ Σ' defs :
+  Forall (fun d => erases_deps Σ Σ' (E.dbody d)) defs ->
+  Forall (erases_deps Σ Σ') (ETyping.fix_subst defs).
+Proof.
+  intros all.
+  unfold ETyping.fix_subst.
+  induction #|defs|; [easy|].
+  cbn in *.
+  constructor; [|easy].
+  constructor.
+  easy.
+Qed.
+
+Lemma erases_deps_eval Σ t v Σ' :
+  Σ' ⊢ t ▷ v ->
+  erases_deps Σ Σ' t ->
+  erases_deps Σ Σ' v.
+Proof.
+  intros ev er.
+  induction ev in t, v, ev, er |- *; cbn in *.
+  - now constructor.
+  - depelim er.
+    apply IHev3.
+    apply erases_deps_csubst; [easy|].
+    intuition auto.
+    now depelim H.
+  - depelim er.
+    now apply IHev2, erases_deps_csubst.
+  - depelim er.
+    apply IHev2.
+    unfold ETyping.iota_red.
+    apply erases_deps_mkApps.
+    + rewrite nth_nth_error.
+      destruct nth_error eqn:nth; [|now constructor].
+      eapply nth_error_forall in nth; [|now eauto].
+      assumption.
+    + intuition auto.
+      apply erases_deps_mkApps_inv in H0.
+      now apply Forall_skipn.
+  - depelim er.
+    subst brs; cbn in *.
+    depelim H0.
+    cbn in *.
+    apply IHev2.
+    apply erases_deps_mkApps; [easy|].
+    apply Forall_repeat.
+    now constructor.
+  - depelim er.
+    intuition auto.
+    eapply erases_deps_mkApps_inv in H0 as (? & ?).
+    depelim H0.
+    apply IHev3.
+    constructor; [|easy].
+    apply erases_deps_mkApps; [|easy].
+    now eapply erases_deps_cunfold_fix.
+  - depelim er.
+    clear H0.
+    intuition auto.
+    apply erases_deps_mkApps_inv in H0 as (? & ?).
+    constructor; [|easy].
+    now apply erases_deps_mkApps.
+  - depelim er.
+    apply erases_deps_mkApps_inv in er as (? & ?).
+    depelim H1.
+    apply IHev.
+    constructor; [|easy].
+    apply erases_deps_mkApps; [|easy].
+    now eapply erases_deps_cunfold_cofix.
+  - depelim er.
+    apply erases_deps_mkApps_inv in er as (? & ?).
+    depelim H0.
+    apply IHev.
+    constructor.
+    apply erases_deps_mkApps; [|easy].
+    now eapply erases_deps_cunfold_cofix.
+  - depelim er.
+    now apply IHev, H3.
+  - depelim er.
+    intuition auto.
+    apply erases_deps_mkApps_inv in H as (? & ?).
+    apply IHev2.
+    rewrite nth_nth_error.
+    destruct nth_error eqn:nth; [|now constructor].
+    now eapply nth_error_forall in nth.
+  - constructor.
+  - depelim er.
+    now constructor.
+  - easy.
+Qed.
+
+Hint Resolve erases_deps_subst1 erases_deps_eval erases_deps_mkApps : core.
+
+Import PA.
+
+Set SsrRewrite.
+Lemma erases_correct Σ t T t' v Σ' :
+  extraction_pre Σ ->
+  Σ;;; [] |- t : T ->
+  Σ;;; [] |- t ⇝ℇ t' ->
+  erases_deps Σ Σ' t' ->
+  Σ |-p t ▷ v ->
+  exists v', Σ;;; [] |- v ⇝ℇ v' /\ Σ' ⊢ t' ▷ v'.
+Proof.
+  intros pre Hty He Heg H.
+  revert T Hty t' He Heg.
+  induction H; intros T Hty t' He Heg; destruct pre as [axfree wfΣ].
+  - assert (Hty' := Hty).
+    assert (eval Σ (PCUICAst.tApp f a) res) by eauto.
+    eapply inversion_App in Hty as (? & ? & ? & ? & ? & ?); eauto.
+    inv He.
+
+    + depelim Heg.
+      eapply IHeval1 in H4 as (vf' & Hvf' & He_vf'); eauto.
+      eapply IHeval2 in H6 as (vu' & Hvu' & He_vu'); eauto.
+      pose proof (subject_reduction_eval t0 H).
+      eapply inversion_Lambda in X0 as (? & ? & ? & ? & ?); eauto.
+      assert (Σ ;;; [] |- a' : t). {
+        eapply subject_reduction_eval; eauto.
+        eapply PCUICConversion.cumul_Prod_inv in c0 as [].
+        econstructor. eassumption. eauto. eapply conv_sym in c0; eauto.
+        now eapply conv_cumul. auto. auto. }
+      assert (eqs := type_closed_subst b wfΣ X0).
+      inv Hvf'.
+      * assert (Σ;;; [] |- PCUICLiftSubst.subst1 a' 0 b ⇝ℇ subst1 vu' 0 t').
+        eapply (erases_subst Σ [] [PCUICAst.vass na t] [] b [a'] t'); eauto.
+        econstructor. econstructor. rewrite parsubst_empty. eassumption.
+        rewrite eqs in H2.
+        eapply IHeval3 in H2 as (v' & Hv' & He_v').
+        -- exists v'. split; eauto.
+           econstructor; eauto.
+           rewrite ECSubst.closed_subst; auto.
+           eapply erases_closed in Hvu'; auto.
+           now eapply PCUICClosed.subject_closed in X0.
+        -- rewrite <-eqs. eapply substitution0; eauto.
+        -- eapply erases_deps_subst1; eauto.
+           eapply erases_deps_eval in He_vf'; eauto.
+           depelim He_vf'.
+           eauto.
+      * exists EAst.tBox. split.
+        eapply Is_type_lambda in X1; eauto. destruct X1. econstructor.
+        eapply (is_type_subst Σ [] [PCUICAst.vass na _] [] _ [a']) in X1 ; auto.
+        cbn in X1.
+        eapply Is_type_eval; try assumption.
+        eauto. eapply H1. rewrite <-eqs. eassumption.
+        all: eauto. econstructor. econstructor. rewrite parsubst_empty.
+        eauto. econstructor. eauto. eauto.
+    + exists EAst.tBox. split. 2:econstructor; eauto.
+      econstructor.
+      eapply Is_type_eval; eauto.
+  - assert (Hty' := Hty).
+    assert (Σ |-p tLetIn na b0 t b1 ▷ res) by eauto.
+    eapply inversion_LetIn in Hty' as (? & ? & ? & ? & ? & ?); auto.
+    inv He.
+    + depelim Heg.
+      eapply IHeval1 in H6 as (vt1' & Hvt2' & He_vt1'); eauto.
+      assert (Hc : PCUICContextConversion.conv_context Σ ([],, vdef na b0 t) [vdef na b0' t]). {
+        econstructor. econstructor. econstructor.
+        eapply PCUICCumulativity.red_conv.
+        now eapply wcbeval_red; eauto.
+        reflexivity.
+      }
+      assert (Σ;;; [vdef na b0' t] |- b1 : x0). {
+        cbn in *. eapply PCUICContextConversion.context_conversion. 3:eauto. all:cbn; eauto.
+        econstructor. all: cbn; eauto. eapply subject_reduction_eval; auto. eauto. eauto.
+      }
+      assert (Σ;;; [] |- PCUICLiftSubst.subst1 b0' 0 b1 ⇝ℇ subst1 vt1' 0 t2'). {
+        eapply (erases_subst Σ [] [PCUICAst.vdef na b0' t] [] b1 [b0'] t2'); eauto.
+        enough (subslet Σ [] [PCUICLiftSubst.subst [] 0 b0'] [vdef na b0' t]).
+        now rewrite parsubst_empty in X1.
+        econstructor. econstructor.
+        rewrite !parsubst_empty.
+        eapply subject_reduction_eval; eauto.
+        eapply erases_context_conversion. 3:eassumption.
+        all: cbn; eauto.
+        econstructor. all: cbn; eauto.
+        eapply subject_reduction_eval; eauto.
+      }
+      unshelve epose proof (subject_reduction_eval t1 H); eauto.
+      assert (eqs := type_closed_subst b1 _ X1).
+      rewrite eqs in H1.
+      eapply IHeval2 in H1 as (vres & Hvres & Hty_vres); eauto.
+      2:{ rewrite <-eqs. eapply substitution_let; eauto. }
+      exists vres. split. eauto. econstructor; eauto.
+      enough (ECSubst.csubst vt1' 0 t2'  = t2' {0 := vt1'}) as ->; auto.
+      eapply ECSubst.closed_subst. eapply erases_closed in Hvt2'; auto.
+      eapply eval_closed. eauto. 2:eauto. now eapply PCUICClosed.subject_closed in t1.
+    + exists EAst.tBox. split. 2:econstructor; eauto.
+      econstructor. eapply Is_type_eval; eauto.
+
+  - destruct Σ as (Σ, univs).
+    assert (Σ |-p tConst c u ▷ res) by eauto.
+    eapply inversion_Const in Hty as (? & ? & ? & ? & ?); [|easy].
+    inv He.
+    + depelim Heg.
+      assert (isdecl' := isdecl).
+      eapply declared_constant_inj in H0; eauto; subst.
+      unfold erases_constant_body in *. rewrite -> e in *.
+      destruct ?; try tauto. cbn in *.
+      eapply declared_constant_inj in d; eauto; subst.
+      edestruct IHeval.
+      * cbn in *.
+        assert (isdecl'' := isdecl').
+        eapply PCUICWeakeningEnv.declared_constant_inv in isdecl'; eauto; try apply wfΣ.
+        2:eapply PCUICWeakeningEnv.weaken_env_prop_typing.
+        unfold on_constant_decl in isdecl'. rewrite e in isdecl'. red in isdecl'.
+        unfold declared_constant in isdecl''.
+        now eapply typing_subst_instance_decl with (Σ0 := (Σ, univs)) (Γ := []); eauto.
+      * assert (isdecl'' := isdecl').
+        eapply PCUICWeakeningEnv.declared_constant_inv in isdecl'; eauto; try apply wfΣ.
+        unfold on_constant_decl in isdecl'. rewrite e in isdecl'. cbn in *.
+        2:eapply PCUICWeakeningEnv.weaken_env_prop_typing.
+        eapply erases_subst_instance_decl with (Σ := (Σ, univs)) (Γ := []); eauto.
+      * apply H3; eauto.
+      * destruct H0. exists x0. split; eauto. econstructor; eauto.
+    + exists EAst.tBox. split. econstructor.
+      eapply Is_type_eval. 3: eassumption. eauto. eauto. eauto. econstructor. eauto.
+
+  - destruct Σ as (Σ, univs).
+    cbn in *.
+    eapply axfree in isdecl. congruence.
+
+  - assert (Hty' := Hty).
+    assert (Σ |-p tCase (ind, pars) p discr brs ▷ res) by eauto.
+    eapply inversion_Case in Hty' as [u' [args' [mdecl [idecl [ps [pty [btys
+                                    [? [? [? [? [? [_ [? [ht0 [? ?]]]]]]]]]]]]]]]]; auto.
+    assert (Σ ;;; [] |- mkApps (tConstruct ind c u) args :  mkApps (tInd ind u') args').
+    eapply subject_reduction_eval; eauto.
+    eapply PCUICValidity.inversion_mkApps in X0 as (? & ? & ?); eauto.
+    eapply inversion_Construct in t1 as (mdecl' & idecl' & cdecl & ? & ? & ? & ?); auto.
+    assert (d1 := d0).
+    destruct d0.
+    edestruct (declared_inductive_inj H1 d). subst.
+    pose proof (@length_of_btys ind mdecl' idecl' (firstn pars args') u' p).
+    pose proof (length_map_option_out _ _ ht0) as lenbtys. simpl in lenbtys.
+    rewrite H3 in lenbtys.
+
+    inv He.
+    + depelim Heg.
+      eapply IHeval1 in H11 as (v' & Hv' & He_v'); eauto.
+      eapply erases_mkApps_inv in Hv' as [(? & ? & ? & ? & [] & ? & ? & ?) | (? & ? & ? & ? & ?)]; eauto.
+      3: eapply subject_reduction_eval; eauto.
+      * subst.
+
+        eapply Is_type_app in X1; auto. destruct X1.
+        2:{ rewrite mkApps_nested. eapply subject_reduction_eval; eauto. }
+        rewrite mkApps_nested in X1.
+
+        eapply tConstruct_no_Type in X1; auto.
+        eapply H10 in X1 as []; eauto. 2: exists []; now destruct Σ.
+
+        destruct (ind_ctors idecl'). cbn in *. destruct c; inv H3.
+        destruct l; cbn in *; try lia. destruct c as [ | []]; cbn in *; inv H3.
+
+        destruct btys as [ | ? []]; cbn in *; try lia. clear H4 lenbtys H5.
+        destruct H8.
+        (* eapply H7 in d1. *) inv a. inv X0.
+        inv X3. inv X4. destruct H8. destruct x3, y; cbn in *; subst.
+        destruct X2. destruct p1; subst; cbn in *.
+        destruct p0 as [narg bty]; simpl in *.
+
+        edestruct (IHeval2) as (? & ? & ?).
+        eapply subject_reduction. eauto. exact Hty.
+        etransitivity.
+        eapply PCUICReduction.red_case_c. eapply wcbeval_red; eauto.
+        econstructor. econstructor. econstructor.
+
+        all:unfold iota_red in *. all:cbn in *.
+        eapply erases_mkApps. eauto.
+        instantiate (1 := repeat EAst.tBox _).
+        eapply All2_Forall2.
+        eapply All2_impl.
+        eapply All2_All_mix_left. eassumption.
+        2:{ intros. destruct X0. assert (y = EAst.tBox). exact y0. subst. econstructor.
+            now eapply isErasable_Proof. }
+
+        eapply All2_right_triv. 2: now rewrite repeat_length.
+        now eapply All_repeat.
+
+        depelim H1.
+        eapply erases_deps_mkApps; [now eauto|].
+        apply Forall_repeat.
+        now constructor.
+
+
+        (* destruct x4; cbn in e2; subst. destruct X2. destruct p0; cbn in e2; subst. cbn in *.  destruct y.  *)
+        exists x3. split; eauto. eapply eval_iota_sing.  2:eauto.
+        pose proof (Ee.eval_to_value _ _ _ He_v').
+        eapply value_app_inv in H5. subst. eassumption.
+
+        eapply wf_ext_wf in wfΣ.
+        eapply tCase_length_branch_inv in wfΣ.
+        2:{ eapply subject_reduction. eauto.
+            exact Hty.
+            eapply PCUICReduction.red_case_c. eapply wcbeval_red; eauto. }
+        2: reflexivity.
+
+        enough (#|skipn (ind_npars mdecl') (x0 ++ x1)| = narg) as <- by eauto.
+        rewrite skipn_length; lia.
+      * subst. unfold iota_red in *.
+        destruct (nth_error brs c) eqn:Hnth.
+        2:{ eapply nth_error_None in Hnth. erewrite All2_length in Hnth. 2:exact a.
+            eapply nth_error_Some_length in H3. cbn in H3. lia. }
+        rewrite <- nth_default_eq in *. unfold nth_default in *.
+        rewrite -> Hnth in *.
+
+        destruct (All2_nth_error_Some _ _ X0 Hnth) as (? & ? & ? & ?).
+        destruct (All2_nth_error_Some _ _ a Hnth) as (? & ? & ? & ?).
+         destruct p0, x3. cbn in *. subst.
+        edestruct IHeval2 as (? & ? & ?).
+        eapply subject_reduction. eauto. exact Hty.
+        etransitivity.
+        eapply PCUICReduction.red_case_c. eapply wcbeval_red. eauto.
+        now eapply PCUICClosed.subject_closed in t0. eauto. eauto.
+
+        etransitivity. eapply trans_red. econstructor.
+        econstructor. unfold iota_red. rewrite <- nth_default_eq. unfold nth_default.
+        rewrite Hnth. econstructor.
+
+        eapply erases_mkApps. eauto.
+        eapply Forall2_skipn. eauto.
+
+        eapply nth_error_forall in H1; [|now eauto].
+        eapply erases_deps_mkApps; [now eauto|].
+        eapply erases_deps_eval in He_v'; [|now eauto].
+        eapply erases_deps_mkApps_inv in He_v' as (? & ?).
+        apply Forall_skipn.
+        now eauto.
+
+        inv H6.
+        -- exists x3. split; eauto.
+           econstructor. eauto. unfold ETyping.iota_red.
+           rewrite <- nth_default_eq. unfold nth_default. rewrite e1. cbn. eauto.
+        -- eapply Is_type_app in X1 as []; auto.
+           2:{ eapply subject_reduction_eval. 2:eassumption. eauto. }
+
+           eapply tConstruct_no_Type in X1; auto.
+           eapply H10 in X1 as []; eauto. 2: exists []; now destruct Σ.
+
+           destruct (ind_ctors idecl'). cbn in *. destruct c; inv H3.
+           destruct l; cbn in *; try lia. destruct c as [ | []]; cbn in *; inv H3.
+
+           destruct btys as [ | ? []]; cbn in *; try discriminate.
+           clear H6. destruct H9.
+            inv a. inv X2. inv X3. inv X0. destruct H11. destruct x0, y; cbn in *; subst.
+           inv X2. destruct p1. subst. destruct p0; cbn in *.
+           destruct X4; subst n1. inv e1. simpl in *. inv Hnth. inv e4. cbn in *.
+
+           edestruct (IHeval2) as (? & ? & ?).
+           eapply subject_reduction. eauto. exact Hty.
+           etransitivity.
+           eapply PCUICReduction.red_case_c. eapply wcbeval_red. eauto.
+           now eapply PCUICClosed.subject_closed in t0; eauto. eauto. eauto.
+           econstructor. econstructor.
+           econstructor.
+
+           eapply erases_mkApps. eauto.
+           instantiate (1 := repeat EAst.tBox _).
+           eapply All2_Forall2.
+           eapply All2_impl.
+           eapply All2_All_mix_left. eassumption.
+           2:{ intros. destruct X0. assert (y = EAst.tBox). exact y0. subst. econstructor.
+               now eapply isErasable_Proof. }
+
+           eapply All2_right_triv. 2:now rewrite repeat_length.
+           now eapply All_repeat.
+
+           depelim H1.
+           eapply erases_deps_mkApps; [now eauto|].
+           eapply Forall_repeat.
+           now constructor.
+
+           exists x0. split; eauto.
+           eapply eval_iota_sing.
+           pose proof (Ee.eval_to_value _ _ _ He_v').
+           2:eauto. auto.
+           apply value_app_inv in H9; subst x1.
+           apply He_v'.
+           enough (#|skipn (ind_npars mdecl') args| = n) as <- by eauto.
+
+           eapply wf_ext_wf in wfΣ.
+           eapply tCase_length_branch_inv in wfΣ.
+           2:{ eapply subject_reduction. eauto.
+               exact Hty.
+               eapply PCUICReduction.red_case_c. eapply wcbeval_red; eauto. }
+           2: reflexivity.
+
+           enough (#|skipn (ind_npars mdecl') args| = n) as <- by eauto.
+           rewrite skipn_length; lia.
+    + exists EAst.tBox. split. econstructor.
+      eapply Is_type_eval; eauto. econstructor; eauto.
+
+  - pose (Hty' := Hty).
+    eapply inversion_Proj in Hty' as (? & ? & ? & [] & ? & ? & ? & ? & ?); [|easy].
+    inv He.
+
+    + depelim Heg.
+      eapply IHeval1 in H5 as (vc' & Hvc' & Hty_vc'); eauto.
+      eapply erases_mkApps_inv in Hvc'; eauto.
+      2: eapply subject_reduction_eval; eauto.
+      destruct Hvc' as [ (? & ? & ? & ? & [] & ? & ? & ?) | (? & ? & ? & ? & ?)]; subst.
+      * exists EAst.tBox. split.
+
+        eapply Is_type_app in X as []; eauto. 2:{ rewrite mkApps_nested. eapply subject_reduction_eval; eauto. }
+        rewrite mkApps_nested in X.
+
+        eapply tConstruct_no_Type in X; eauto. eapply H3 in X as [? []]; eauto.
+        2: now destruct d. 2: now exists []; destruct Σ.
+
+        econstructor.
+        eapply Is_type_eval; eauto. eauto.
+        eapply nth_error_all.
+        erewrite nth_error_skipn. reflexivity. eassumption.
+        eapply All_impl. assert (pars = ind_npars x0). destruct d as (? & ? & ?). now rewrite H7. subst.
+        eassumption.
+        eapply isErasable_Proof. eauto.
+
+        eapply eval_proj_box.
+        pose proof (Ee.eval_to_value _ _ _ Hty_vc').
+        eapply value_app_inv in H1. subst. eassumption.
+      * rename H3 into Hinf.
+        eapply Forall2_nth_error_Some in H4 as (? & ? & ?); eauto.
+        assert (Σ ;;; [] |- mkApps (tConstruct i 0 u) args : mkApps (tInd i x) x2).
+        eapply subject_reduction_eval; eauto.
+        eapply PCUICValidity.inversion_mkApps in X as (? & ? & ?); eauto.
+        eapply typing_spine_inv in t2 as []; eauto.
+        eapply IHeval2 in H3 as (? & ? & ?); eauto.
+        inv H2.
+        -- exists x8. split; eauto. econstructor. eauto.
+           rewrite <- nth_default_eq. unfold nth_default. now rewrite H1.
+        -- exists EAst.tBox. split.
+
+
+           eapply Is_type_app in X as []; eauto. 2:{ eapply subject_reduction_eval; [|eauto]; eauto. }
+
+           eapply tConstruct_no_Type in X. eapply Hinf in X as [? []]; eauto.
+           2: now destruct d. 2: now exists []; destruct Σ.
+
+           econstructor.
+           eapply Is_type_eval; eauto.
+           eapply nth_error_all.
+           erewrite nth_error_skipn. reflexivity. eassumption.
+           eapply All_impl. assert (pars = ind_npars x0). destruct d as (? & ? & ?). now rewrite H7. subst.
+           eassumption.
+           eapply isErasable_Proof. eauto.
+
+           eapply eval_proj_box.
+           pose proof (Ee.eval_to_value _ _ _ Hty_vc').
+           eapply value_app_inv in H2. subst. eassumption.
+        -- eapply erases_deps_eval in Hty_vc'; [|now eauto].
+           eapply erases_deps_mkApps_inv in Hty_vc' as (? & ?).
+           now eapply nth_error_forall in H1; eauto.
+    + exists EAst.tBox. split. econstructor.
+      eapply Is_type_eval. 4: eassumption. all: eauto. econstructor. eauto.
+
+  - assert (Hty' := Hty).
+    assert (Hunf := H).
+    assert (Hcon := H1).
+    eapply inversion_App in Hty' as (? & ? & ? & ? & ? & ?); eauto.
+    assert (Ht := t).
+    eapply subject_reduction in t. 2:auto. 2:eapply wcbeval_red; eauto.
+    assert (HT := t).
+    apply PCUICValidity.inversion_mkApps in HT as (? & ? & ?); auto.
+    assert (Ht1 := t1).
+    apply inversion_Fix in t1 as Hfix; auto.
+    destruct Hfix as (? & ? & ? & ? & ? & ? & ?).
+    unfold cunfold_fix in e. rewrite e0 in e. inv e.
+    depelim He; first last.
+
+    + exists EAst.tBox. split; [|now constructor].
+      econstructor.
+      eapply Is_type_eval. 4:eapply X. eauto. eauto.
+      eapply eval_fix; eauto.
+      rewrite /cunfold_fix e0 //. congruence.
+    + depelim Heg.
+      eapply IHeval1 in He1 as IH1; eauto.
+      destruct IH1 as (er_stuck_v & er_stuck & ev_stuck).
+      eapply IHeval2 in He2 as IH2; eauto.
+      destruct IH2 as (er_argv & er_arg & ev_arg).
+      eapply erases_mkApps_inv in er_stuck; eauto.
+      destruct er_stuck as [(? & ? & ? & -> & ? & ? & ? & ->)|
+                            (? & ? & -> & ? & ?)].
+      { exists E.tBox.
+        eapply eval_to_mkApps_tBox_inv in ev_stuck as ?; subst.
+        cbn in *.
+        split; [|eauto using Ee.eval].
+        destruct H2.
+        eapply (Is_type_app _ _ _ (x5 ++ [av])) in X as []; eauto; first last.
+        - rewrite mkApps_nested app_assoc mkApps_snoc.
+          eapply type_App; eauto.
+          eapply subject_reduction; eauto.
+          eapply wcbeval_red; eauto.
+        - eapply erases_box.
+          eapply Is_type_eval; auto. 2:eauto.
+          rewrite -mkApps_nested /=.
+          eapply eval_fix.
+          rewrite mkApps_nested. eapply value_final.
+          eapply eval_to_value; eauto.
+          eapply value_final, eval_to_value; eauto.
+          rewrite  /cunfold_fix e0 //. auto. auto.
+          rewrite H3; eauto. auto. }
+
+      inv H2.
+      * assert (Hmfix' := X).
+        eapply All2_nth_error_Some in X as (? & ? & ?); eauto.
+        pose proof (closed_fix_substl_subst_eq (PCUICClosed.subject_closed _ t1) e0) as cls.
+        destruct x3. cbn in *. subst.
+
+        enough (Σ;;; [] ,,, PCUICLiftSubst.subst_context (fix_subst mfix) 0 []
+                |- PCUICLiftSubst.subst (fix_subst mfix) 0 dbody
+                ⇝ℇ subst (ETyping.fix_subst mfix') 0 (Extract.E.dbody x4)).
+        destruct p. destruct p.
+
+        clear e3. rename H into e3.
+        -- cbn in e3. rename x5 into L.
+           eapply (erases_mkApps _ _ _ _ (argsv ++ [av])) in H2; first last.
+           { eapply Forall2_app.
+             - exact H4.
+             - eauto. }
+           rewrite <- mkApps_nested in H2.
+           rewrite EAstUtils.mkApps_app in H2.
+           cbn in *. simpl in H2.
+           rewrite cls in H2.
+           eapply IHeval3 in H2 as (? & ? & ?); cbn; eauto; cycle 1.
+           { eapply subject_reduction. eauto. exact Hty.
+             etransitivity.
+             eapply PCUICReduction.red_app. eapply wcbeval_red; eauto.
+             eapply wcbeval_red; eauto.
+             rewrite <- !mkApps_snoc.
+             eapply PCUICReduction.red1_red.
+             eapply red_fix.
+             rewrite closed_unfold_fix_cunfold_eq.
+             now eapply PCUICClosed.subject_closed in t1.
+             rewrite /cunfold_fix e0 /= //.
+             pose proof (eval_to_value _ _ _ e3) as vfix.
+             eapply PCUICWcbvEval.stuck_fix_value_args in vfix; eauto.
+             2:{ rewrite /cunfold_fix e0 //. }
+             simpl in vfix.
+             subst. unfold is_constructor.
+             rewrite nth_error_snoc. lia.
+             assert(Σ ;;; [] |- mkApps (tFix mfix idx) (argsv ++ [av]) : PCUICLiftSubst.subst [av] 0 x1).
+             { rewrite -mkApps_nested. eapply type_App; eauto. eapply subject_reduction_eval;eauto. }
+             epose proof (fix_app_is_constructor Σ (args:=argsv ++ [av])%list axfree X).
+             rewrite /unfold_fix e0 in X0.
+             specialize (X0 eq_refl). simpl in X0.
+             rewrite nth_error_snoc in X0. auto. apply X0.
+             eapply value_whnf; eauto.
+             eapply eval_closed; eauto. now eapply PCUICClosed.subject_closed in t0.
+             eapply eval_to_value; eauto. }
+
+           { constructor.
+             - eapply erases_deps_eval in ev_stuck; [|now eauto].
+               eapply erases_deps_mkApps_inv in ev_stuck as (? & ?).
+               apply erases_deps_mkApps; [|now eauto].
+               depelim H.
+               eapply nth_error_forall in H as H'; eauto.
+               apply erases_deps_subst; [|now eauto].
+               now apply Forall_All, erases_deps_fix_subst; eauto.
+             - now eapply erases_deps_eval in ev_arg; eauto. }
+
+           exists x3. split. eauto.
+           eapply Ee.eval_fix.
+           ++ eauto.
+           ++ eauto.
+           ++ rewrite <- Ee.closed_unfold_fix_cunfold_eq.
+              { unfold ETyping.unfold_fix. rewrite e -e2.
+                now rewrite (Forall2_length H4). }
+              eapply eval_closed in e3; eauto.
+              clear -e3 Hmfix'.
+              pose proof (All2_length _ _ Hmfix').
+              eapply PCUICClosed.closedn_mkApps_inv in e3.
+              apply andb_true_iff in e3 as (e3 & _).
+              change (?a = true) with (is_true a) in e3.
+              simpl in e3 |- *. solve_all.
+              rewrite app_context_nil_l in b.
+              eapply erases_closed in b. simpl in b.
+              rewrite <- H.
+              unfold EAst.test_def.
+              simpl in b.
+              rewrite fix_context_length in b.
+              now rewrite Nat.add_0_r.
+              unfold test_def in a. apply andP in a as [_ Hbod].
+              rewrite fix_context_length.
+              now rewrite Nat.add_0_r in Hbod.
+              eauto with pcuic.
+              now eapply PCUICClosed.subject_closed in Ht.
+           ++ auto.
+        -- cbn. destruct p. destruct p.
+           eapply (erases_subst Σ [] (PCUICLiftSubst.fix_context mfix) [] dbody (fix_subst mfix)) in e3; cbn; eauto.
+           ++ eapply subslet_fix_subst. now eapply wf_ext_wf. all: eassumption.
+           ++ eapply nth_error_all in a1; eauto. cbn in a1.
+              eapply a1.
+           ++ eapply All2_from_nth_error.
+              erewrite fix_subst_length, ETyping.fix_subst_length, All2_length; eauto.
+              intros.
+              rewrite fix_subst_nth in H3. now rewrite fix_subst_length in H2.
+              rewrite efix_subst_nth in H5. rewrite fix_subst_length in H2.
+              erewrite <- All2_length; eauto.
+              inv H5; inv H3.
+              erewrite All2_length; eauto.
+      * eapply (Is_type_app _ _ _ (argsv ++ [av])) in X as []; tas.
+        -- exists EAst.tBox.
+           split.
+           ++ econstructor.
+              eapply Is_type_eval. 4:eauto. all:eauto.
+              rewrite -mkApps_nested.
+              eapply eval_fix; eauto.
+              1-2:eapply value_final, eval_to_value; eauto.
+              rewrite /cunfold_fix e0 //. congruence.
+           ++ eapply Ee.eval_box; [|eauto].
+              apply eval_to_mkApps_tBox_inv in ev_stuck as ?; subst.
+              eauto.
+        -- eauto.
+        -- rewrite mkApps_snoc.
+           eapply type_App; eauto.
+           eapply subject_reduction; eauto.
+           eapply wcbeval_red; eauto.
+
+  - apply inversion_App in Hty as Hty'; [|eauto].
+    destruct Hty' as (? & ? & ? & ? & ? & ?).
+
+    eapply subject_reduction in t as typ_stuck_fix; [|eauto|]; first last.
+    { eapply wcbeval_red. 4: eauto. all: eauto. }
+
+    eapply erases_App in He as He'; [|eauto].
+    destruct He' as [(-> & [])|(? & ? & -> & ? & ?)].
+    + exists E.tBox.
+      split; [|eauto using Ee.eval].
+      constructor.
+      eapply Is_type_red.
+      * eauto.
+      * eapply PCUICReduction.red_app.
+        -- eapply wcbeval_red; [eauto|eauto| |eauto]. eauto.
+        -- eapply wcbeval_red; [eauto|eauto| |eauto]. eauto.
+      * eauto.
+    + depelim Heg.
+      eapply subject_reduction in t0 as typ_arg; [|eauto|]; first last.
+      { eapply wcbeval_red; [eauto|eauto| |eauto]. eauto. }
+
+      eapply IHeval1 in H1 as (? & ? & ?); [|now eauto|now eauto].
+      eapply IHeval2 in H2 as (? & ? & ?); [|now eauto|now eauto].
+      eapply erases_mkApps_inv in H1; [|eauto|eauto].
+      destruct H1 as [(? & ? & ? & -> & [] & ? & ? & ->)|(? & ? & -> & ? & ?)].
+      * apply eval_to_mkApps_tBox_inv in H3 as ?; subst.
+        depelim H5.
+        rewrite -> !app_nil_r in *.
+        cbn in *.
+        exists E.tBox.
+        split; [|eauto using Ee.eval].
+        eapply (Is_type_app _ _ _ [av]) in X as [].
+        -- constructor.
+           apply X.
+        -- eauto.
+        -- eauto.
+        -- cbn.
+           eapply type_App; eauto.
+      * depelim H1.
+        -- exists (E.tApp (E.mkApps (E.tFix mfix' idx) x7) x5).
+           split; [eauto using erases_tApp, erases_mkApps|].
+           unfold cunfold_fix in *.
+           destruct (nth_error _ _) eqn:nth; [|congruence].
+           eapply All2_nth_error_Some in X as (? & ? & ? & ? & ?); [|eauto].
+           eapply Ee.eval_fix_value.
+           ++ eauto.
+           ++ eauto.
+           ++ unfold Ee.cunfold_fix.
+              rewrite e0.
+              reflexivity.
+           ++ eapply Forall2_length in H5. noconf e. lia.
+
+        -- exists E.tBox.
+           apply eval_to_mkApps_tBox_inv in H3 as ?; subst.
+           split; [|eauto using Ee.eval].
+           eapply Is_type_app in X as [].
+           ++ constructor.
+              rewrite <- mkApps_snoc.
+              exact X.
+           ++ eauto.
+           ++ eauto.
+           ++ rewrite mkApps_snoc.
+              eapply type_App; eauto.
+
+  - destruct ip.
+    assert (Hty' := Hty).
+    eapply inversion_Case in Hty' as [u' [args' [mdecl [idecl [ps [pty [btys
+                                   [? [? [? [? [? [_ [? [ht0 [? ?]]]]]]]]]]]]]]]];
+    eauto.
+    eapply PCUICValidity.inversion_mkApps in t0 as (? & ? & ?); eauto.
+    eapply inversion_CoFix in t0 as (? & ? & ? &?); eauto.
+    todo "erasure cofix"%string.
+
+  - assert (Hty' := Hty).
+    eapply inversion_Proj in Hty' as (? & ? & ? & [] & ? & ? & ? & ? & ?).
+    eapply PCUICValidity.inversion_mkApps in t0 as (? & ? & ?); eauto.
+    eapply inversion_CoFix in t0 as (? & ? & ? &?); eauto.
+    todo "erasure cofix". auto.
+  - pose (Hty' := Hty).
+    eapply inversion_App in Hty' as (? & ? & ? & ? & ? & ?); eauto.
+    inv He.
+    + depelim Heg.
+      assert (t' := t). eapply IHeval1 in t as (? & ? & ?); eauto.
+      eapply IHeval2 in t0 as (? & ? & ?); eauto.
+      destruct (EAstUtils.isBox x2) eqn:E.
+      * destruct x2; inv E. exists EAst.tBox. split. 2: econstructor; eauto.
+        pose proof (Is_type_app Σ [] f'[a']).
+        inversion H1.
+        edestruct H7; eauto. cbn. eapply subject_reduction. eauto.
+        exact Hty. eapply PCUICReduction.red_app.
+        eapply wcbeval_red; eauto.
+        eapply inversion_App in Hty as [na [A [B [Hf [Ha _]]]]]; eauto.
+        eapply wcbeval_red; eauto.
+      * exists (E.tApp x2 x3).
+        split. 2:{ eapply Ee.eval_app_cong; eauto.
+                   eapply ssrbool.negbT.
+                   repeat eapply orb_false_intro.
+                   - destruct x2; try reflexivity.
+                     inv H1. inv i.
+                   - destruct x2 eqn:Ex; try reflexivity.
+                     + cbn. inv H1. cbn in *.
+                       eapply ssrbool.negbTE, is_FixApp_erases.
+                       econstructor; eauto.
+                       now rewrite orb_false_r in i.
+                     + cbn in *.
+                       inv H1. inv i.
+                   - eauto. }
+        econstructor; eauto.
+    + exists EAst.tBox. split. 2: now econstructor.
+      econstructor.
+      eapply inversion_App in Hty as [na [A [B [Hf [Ha _]]]]]; auto.
+      eapply Is_type_red. 3:eauto. eauto.
+      eapply PCUICReduction.red_app.
+      eapply PCUICClosed.subject_closed in Hf; auto.
+      eapply wcbeval_red; eauto.
+      eapply PCUICClosed.subject_closed in Ha; auto.
+      eapply wcbeval_red; eauto.
+
+  - destruct t; try easy.
+    + inv He. eexists. split; eauto. now econstructor.
+    + inv He. eexists. split; eauto. now econstructor.
+    + inv He.
+      * eexists. split; eauto. now econstructor.
+      * eexists. split. 2: now econstructor.
+        econstructor; eauto.
+    + inv He.
+      * eexists. split. 2: now econstructor.
+        econstructor; eauto.
+    + inv He.
+      * eexists. split. 2: now econstructor.
+        econstructor; eauto.
+      * eexists. split. 2: now econstructor.
+        eauto.
+    + inv He.
+      * eexists. split; eauto. now econstructor.
+      * eexists. split. 2: now econstructor.
+        econstructor; eauto.
+    + inv He.
+      * eexists. split; eauto. now econstructor.
+      * eexists. split. 2: now econstructor.
+        econstructor; eauto.
+Qed.
